<?xml version="1.0" encoding="utf-8"?>
<rdf:RDF
   xmlns:dcterms="http://purl.org/dc/terms/"
   xmlns:ns1="https://m82-project.org/dima-bias/ontology#"
   xmlns:owl="http://www.w3.org/2002/07/owl#"
   xmlns:rdf="http://www.w3.org/1999/02/22-rdf-syntax-ns#"
   xmlns:rdfs="http://www.w3.org/2000/01/rdf-schema#"
>
  <rdf:Description rdf:about="https://stratcomcoe.org/influence-mini/ontology#c9ce7d9bb7_premise_3">
    <ns1:usesTechnique rdf:resource="https://m82-project.org/dima-bias/ontology#c9ce7d9bb7_negativitybias_1"/>
  </rdf:Description>
  <rdf:Description rdf:nodeID="N380ad3e10604473f9422c50c47973d2c">
    <owl:someValuesFrom rdf:resource="https://m82-project.org/dima-bias/ontology#Detect"/>
    <rdf:type rdf:resource="http://www.w3.org/2002/07/owl#Restriction"/>
    <owl:onProperty rdf:resource="https://m82-project.org/dima-bias/ontology#isTacticOf"/>
  </rdf:Description>
  <rdf:Description rdf:about="https://m82-project.org/dima-bias/ontology#DetectTechnique">
    <rdfs:comment xml:lang="en">Techniques that belong to Detect‑phase tactics.</rdfs:comment>
    <rdfs:label xml:lang="en">Detect technique</rdfs:label>
    <rdfs:subClassOf rdf:resource="https://m82-project.org/dima-bias/ontology#Technique"/>
    <rdfs:subClassOf rdf:nodeID="Nd3fafb67c04f43dea9a78f012967ae24"/>
    <rdfs:subClassOf rdf:nodeID="N153767bfc4ce4886a7dbc593be53478d"/>
    <rdf:type rdf:resource="http://www.w3.org/2002/07/owl#Class"/>
  </rdf:Description>
  <rdf:Description rdf:about="https://m82-project.org/dima-bias/ontology#IllusorySuperiority">
    <rdfs:subClassOf rdf:resource="https://m82-project.org/dima-bias/ontology#ActTechnique"/>
    <rdf:type rdf:resource="http://www.w3.org/2002/07/owl#NamedIndividual"/>
    <rdf:type rdf:resource="https://m82-project.org/dima-bias/ontology#Technique"/>
    <rdf:type rdf:resource="https://m82-project.org/dima-bias/ontology#ActTechnique"/>
    <rdf:type rdf:resource="http://www.w3.org/2002/07/owl#Class"/>
    <rdfs:comment xml:lang="en">Belief that one is better than others, often unrealistically.</rdfs:comment>
    <rdfs:comment xml:lang="fr">Croyance que l’on est meilleur que les autres, souvent à tort.</rdfs:comment>
    <rdfs:label xml:lang="en">illusory superiority</rdfs:label>
    <rdfs:label xml:lang="fr">Supériorité illusoire</rdfs:label>
    <ns1:valueCode rdf:datatype="http://www.w3.org/2001/XMLSchema#string">TE0413</ns1:valueCode>
  </rdf:Description>
  <rdf:Description rdf:nodeID="Nb7abcfaf46464d3e82c7ee49bacb1903">
    <rdf:first rdf:resource="https://stratcomcoe.org/influence-mini/ontology#Argument"/>
    <rdf:rest rdf:nodeID="Nf6622a7a9046414dbe83069585aecb6d"/>
  </rdf:Description>
  <rdf:Description rdf:about="https://m82-project.org/dima-bias/ontology#PeltzmanEffect">
    <rdfs:comment xml:lang="en">Tendency to take greater risks when one feels protected.</rdfs:comment>
    <rdfs:comment xml:lang="fr">Tendance à prendre plus de risques en se sentant protégé.</rdfs:comment>
    <rdf:type rdf:resource="https://m82-project.org/dima-bias/ontology#Technique"/>
    <rdf:type rdf:resource="https://m82-project.org/dima-bias/ontology#ActTechnique"/>
    <rdf:type rdf:resource="http://www.w3.org/2002/07/owl#Class"/>
    <rdf:type rdf:resource="http://www.w3.org/2002/07/owl#NamedIndividual"/>
    <rdfs:subClassOf rdf:resource="https://m82-project.org/dima-bias/ontology#ActTechnique"/>
    <rdfs:label xml:lang="fr">Effet Peltzman (compensation du risque)</rdfs:label>
    <rdfs:label xml:lang="en">Peltzman effect</rdfs:label>
    <ns1:valueCode rdf:datatype="http://www.w3.org/2001/XMLSchema#string">TE0412</ns1:valueCode>
  </rdf:Description>
  <rdf:Description rdf:about="https://m82-project.org/dima-bias/ontology#StatusQuoBias">
    <ns1:valueCode rdf:datatype="http://www.w3.org/2001/XMLSchema#string">TE0432</ns1:valueCode>
    <rdfs:comment xml:lang="en">Preference for keeping things as they are, avoiding change.</rdfs:comment>
    <rdfs:comment xml:lang="fr">Préférence pour le statu quo même si d'autres options sont meilleures.</rdfs:comment>
    <rdfs:label xml:lang="en">status quo bias</rdfs:label>
    <rdfs:label xml:lang="fr">Biais du statu quo</rdfs:label>
    <rdf:type rdf:resource="http://www.w3.org/2002/07/owl#Class"/>
    <rdf:type rdf:resource="http://www.w3.org/2002/07/owl#NamedIndividual"/>
    <rdf:type rdf:resource="https://m82-project.org/dima-bias/ontology#ActTechnique"/>
    <rdf:type rdf:resource="https://m82-project.org/dima-bias/ontology#Technique"/>
    <rdfs:subClassOf rdf:resource="https://m82-project.org/dima-bias/ontology#ActTechnique"/>
  </rdf:Description>
  <rdf:Description rdf:about="https://m82-project.org/dima-bias/ontology#ContextEffect_Memorise">
    <rdfs:subClassOf rdf:resource="https://m82-project.org/dima-bias/ontology#MemoriseTechnique"/>
    <rdf:type rdf:resource="http://www.w3.org/2002/07/owl#NamedIndividual"/>
    <rdf:type rdf:resource="https://m82-project.org/dima-bias/ontology#Technique"/>
    <rdf:type rdf:resource="https://m82-project.org/dima-bias/ontology#MemoriseTechnique"/>
    <rdf:type rdf:resource="http://www.w3.org/2002/07/owl#Class"/>
    <rdfs:label xml:lang="en">context effect</rdfs:label>
    <rdfs:label xml:lang="fr">Effet de contexte</rdfs:label>
    <rdfs:comment xml:lang="fr">La mémorisation est affectée par le contexte environnemental ou émotionnel.</rdfs:comment>
    <rdfs:comment xml:lang="en">Memory is influenced by environmental or emotional context.</rdfs:comment>
    <ns1:valueCode rdf:datatype="http://www.w3.org/2001/XMLSchema#string">TE0323</ns1:valueCode>
  </rdf:Description>
  <rdf:Description rdf:about="https://m82-project.org/dima-bias/ontology#ActTactic">
    <rdfs:label xml:lang="en">Act tactic</rdfs:label>
    <rdf:type rdf:resource="http://www.w3.org/2002/07/owl#Class"/>
    <rdfs:subClassOf rdf:resource="https://m82-project.org/dima-bias/ontology#Tactic"/>
    <rdfs:subClassOf rdf:nodeID="N520932e1769f4f768078c62acb1eaa8d"/>
    <rdfs:subClassOf rdf:nodeID="Na4b452aee43c4317a1a113980770d9e4"/>
    <rdfs:comment xml:lang="en">Tactics associated with the Act phase.</rdfs:comment>
  </rdf:Description>
  <rdf:Description rdf:about="https://m82-project.org/dima-bias/ontology#OverconfidenceBias">
    <rdf:type rdf:resource="http://www.w3.org/2002/07/owl#Class"/>
    <rdf:type rdf:resource="http://www.w3.org/2002/07/owl#NamedIndividual"/>
    <rdf:type rdf:resource="https://m82-project.org/dima-bias/ontology#ActTechnique"/>
    <rdf:type rdf:resource="https://m82-project.org/dima-bias/ontology#Technique"/>
    <ns1:valueCode rdf:datatype="http://www.w3.org/2001/XMLSchema#string">TE0411</ns1:valueCode>
    <rdfs:label xml:lang="fr">biais d'excès de confiance</rdfs:label>
    <rdfs:label xml:lang="en">overconfidence bias</rdfs:label>
    <rdfs:subClassOf rdf:resource="https://m82-project.org/dima-bias/ontology#ActTechnique"/>
    <rdfs:comment xml:lang="en">Overestimating one's abilities, performance, or judgment.</rdfs:comment>
    <rdfs:comment xml:lang="fr">Surestimer ses compétences, sa performance ou son jugement.</rdfs:comment>
  </rdf:Description>
  <rdf:Description rdf:nodeID="N10a1167eb3a34bd384b68503c6412474">
    <rdf:first rdf:resource="https://m82-project.org/dima-bias/ontology#usesTechnique"/>
    <rdf:rest rdf:nodeID="N182955c727594ac287dfefec74b37386"/>
  </rdf:Description>
  <rdf:Description rdf:nodeID="N2292c5effbe645e49efbaefd7a3f526f">
    <rdf:type rdf:resource="http://www.w3.org/2002/07/owl#Restriction"/>
    <owl:hasValue rdf:resource="https://m82-project.org/dima-bias/ontology#Detect"/>
    <owl:onProperty rdf:resource="https://m82-project.org/dima-bias/ontology#usesPhase"/>
  </rdf:Description>
  <rdf:Description rdf:about="https://m82-project.org/dima-bias/ontology#ZeroSumBias">
    <rdf:type rdf:resource="https://m82-project.org/dima-bias/ontology#InformTechnique"/>
    <rdf:type rdf:resource="https://m82-project.org/dima-bias/ontology#Technique"/>
    <rdf:type rdf:resource="http://www.w3.org/2002/07/owl#Class"/>
    <rdf:type rdf:resource="http://www.w3.org/2002/07/owl#NamedIndividual"/>
    <rdfs:label xml:lang="en">zero-sum bias</rdfs:label>
    <rdfs:label xml:lang="fr">Biais de la somme nulle</rdfs:label>
    <ns1:valueCode rdf:datatype="http://www.w3.org/2001/XMLSchema#string">TE0241</ns1:valueCode>
    <rdfs:subClassOf rdf:resource="https://m82-project.org/dima-bias/ontology#InformTechnique"/>
    <rdfs:comment xml:lang="fr">Croire que le gain de l’un implique la perte de l’autre.</rdfs:comment>
    <rdfs:comment xml:lang="en">Believing that gains for others mean losses for oneself.</rdfs:comment>
  </rdf:Description>
  <rdf:Description rdf:about="https://m82-project.org/dima-bias/ontology#c9ce7d9bb7_vonrestorffeffect_0">
    <rdf:type rdf:resource="http://www.w3.org/2002/07/owl#NamedIndividual"/>
    <rdf:type rdf:resource="https://m82-project.org/dima-bias/ontology#TechniqueUsage"/>
    <ns1:instantiatesTechnique rdf:resource="https://m82-project.org/dima-bias/ontology#VonRestorffEffect"/>
    <ns1:hasExplanation rdf:datatype="http://www.w3.org/2001/XMLSchema#string">The argument isolates Caldria as uniquely stabilizing and commendable amid volatility and inflammatory actions, making its role stand out and be more memorable by contrast with its environment.</ns1:hasExplanation>
  </rdf:Description>
  <rdf:Description rdf:about="https://m82-project.org/dima-bias/ontology#WeberFechnerLaw">
    <rdf:type rdf:resource="https://m82-project.org/dima-bias/ontology#DetectTechnique"/>
    <rdf:type rdf:resource="http://www.w3.org/2002/07/owl#Class"/>
    <rdf:type rdf:resource="http://www.w3.org/2002/07/owl#NamedIndividual"/>
    <rdf:type rdf:resource="https://m82-project.org/dima-bias/ontology#Technique"/>
    <rdfs:label xml:lang="fr">Loi de Weber-Fechner</rdfs:label>
    <rdfs:label xml:lang="en">Weber-Fechner law</rdfs:label>
    <ns1:valueCode rdf:datatype="http://www.w3.org/2001/XMLSchema#string">TE0152</ns1:valueCode>
    <rdfs:subClassOf rdf:resource="https://m82-project.org/dima-bias/ontology#DetectTechnique"/>
    <rdfs:comment xml:lang="fr">Plus un stimulus est intense, plus il faut de changement pour percevoir une différence.</rdfs:comment>
    <rdfs:comment xml:lang="en">Perception of change depends on relative—not absolute—stimulus intensity.</rdfs:comment>
  </rdf:Description>
  <rdf:Description rdf:about="https://m82-project.org/dima-bias/ontology#IndividualValorisation">
    <ns1:valueCode rdf:datatype="http://www.w3.org/2001/XMLSchema#string">TA0041</ns1:valueCode>
    <rdf:type rdf:resource="http://www.w3.org/2002/07/owl#Class"/>
    <rdf:type rdf:resource="http://www.w3.org/2002/07/owl#NamedIndividual"/>
    <rdf:type rdf:resource="https://m82-project.org/dima-bias/ontology#ActTactic"/>
    <rdf:type rdf:resource="https://m82-project.org/dima-bias/ontology#Tactic"/>
    <rdfs:comment xml:lang="fr">Tactique qui valorise le jugement personnel et la confiance en soi.</rdfs:comment>
    <rdfs:comment xml:lang="en">A tactic that emphasizes personal judgment and self-confidence.</rdfs:comment>
    <ns1:hasTechnique rdf:resource="https://m82-project.org/dima-bias/ontology#OverconfidenceBias"/>
    <ns1:hasTechnique rdf:resource="https://m82-project.org/dima-bias/ontology#IllusorySuperiority"/>
    <ns1:hasTechnique rdf:resource="https://m82-project.org/dima-bias/ontology#PeltzmanEffect"/>
    <rdfs:label xml:lang="fr">Valorisation individuelle</rdfs:label>
    <rdfs:label xml:lang="en">Individual valorisation</rdfs:label>
    <rdfs:subClassOf rdf:resource="https://m82-project.org/dima-bias/ontology#ActTactic"/>
  </rdf:Description>
  <rdf:Description rdf:about="https://m82-project.org/dima-bias/ontology#SpacingEffect">
    <rdfs:label xml:lang="en">spacing effect</rdfs:label>
    <rdfs:label xml:lang="fr">effet d'espacement</rdfs:label>
    <rdf:type rdf:resource="https://m82-project.org/dima-bias/ontology#Technique"/>
    <rdf:type rdf:resource="http://www.w3.org/2002/07/owl#NamedIndividual"/>
    <rdf:type rdf:resource="https://m82-project.org/dima-bias/ontology#MemoriseTechnique"/>
    <rdf:type rdf:resource="http://www.w3.org/2002/07/owl#Class"/>
    <ns1:valueCode rdf:datatype="http://www.w3.org/2001/XMLSchema#string">TE0313</ns1:valueCode>
    <rdfs:comment xml:lang="fr">Mémorisation renforcée grâce à une exposition répétée avec des intervalles de temps.</rdfs:comment>
    <rdfs:comment xml:lang="en">Improved memory retention when learning is spaced over time.</rdfs:comment>
    <rdfs:subClassOf rdf:resource="https://m82-project.org/dima-bias/ontology#MemoriseTechnique"/>
  </rdf:Description>
  <rdf:Description rdf:about="https://m82-project.org/dima-bias/ontology#hasTactic">
    <rdfs:label xml:lang="fr">possède une tactique</rdfs:label>
    <rdfs:label xml:lang="en">has tactic</rdfs:label>
    <rdfs:comment xml:lang="en">Associates a narrative tactic with a DIMA phase (Detect, Inform, etc.).</rdfs:comment>
    <rdfs:comment xml:lang="fr">Associe une tactique narrative à une phase DIMA (Détecter, Informer, etc.).</rdfs:comment>
    <rdf:type rdf:resource="http://www.w3.org/2002/07/owl#ObjectProperty"/>
    <rdfs:range rdf:resource="https://m82-project.org/dima-bias/ontology#Tactic"/>
    <rdfs:domain rdf:resource="https://m82-project.org/dima-bias/ontology#Phase"/>
  </rdf:Description>
  <rdf:Description rdf:about="https://m82-project.org/dima-bias/ontology#MemoriseArgument">
    <rdfs:label xml:lang="en">Memorise argument</rdfs:label>
    <owl:equivalentClass rdf:nodeID="N1029932e0a2f49df875a9ee49ab55619"/>
    <owl:equivalentClass rdf:nodeID="Nac059f911837400bba42ea6c55e0a51d"/>
    <rdf:type rdf:resource="http://www.w3.org/2002/07/owl#Class"/>
    <rdfs:comment xml:lang="en">Arguments that use techniques from the Memorise phase.</rdfs:comment>
  </rdf:Description>
  <rdf:Description rdf:about="https://m82-project.org/dima-bias/ontology#HindsightBias">
    <rdfs:comment xml:lang="en">Believing events were more predictable after they happened.</rdfs:comment>
    <rdfs:comment xml:lang="fr">Croire qu’un événement était prévisible après qu’il se soit produit.</rdfs:comment>
    <rdf:type rdf:resource="https://m82-project.org/dima-bias/ontology#Technique"/>
    <rdf:type rdf:resource="https://m82-project.org/dima-bias/ontology#InformTechnique"/>
    <rdf:type rdf:resource="http://www.w3.org/2002/07/owl#Class"/>
    <rdf:type rdf:resource="http://www.w3.org/2002/07/owl#NamedIndividual"/>
    <rdfs:subClassOf rdf:resource="https://m82-project.org/dima-bias/ontology#InformTechnique"/>
    <rdfs:label xml:lang="fr">Biais rétrospectif</rdfs:label>
    <rdfs:label xml:lang="en">hindsight bias</rdfs:label>
    <ns1:valueCode rdf:datatype="http://www.w3.org/2001/XMLSchema#string">TE0261</ns1:valueCode>
  </rdf:Description>
  <rdf:Description rdf:about="https://m82-project.org/dima-bias/ontology#SourceConfusionBias">
    <rdfs:comment xml:lang="en">Confusing the source of a memory, attributing it incorrectly.</rdfs:comment>
    <rdfs:comment xml:lang="fr">Confusion entre la source d'un souvenir réel et une information extérieure.</rdfs:comment>
    <rdf:type rdf:resource="https://m82-project.org/dima-bias/ontology#MemoriseTechnique"/>
    <rdf:type rdf:resource="http://www.w3.org/2002/07/owl#Class"/>
    <rdf:type rdf:resource="http://www.w3.org/2002/07/owl#NamedIndividual"/>
    <rdf:type rdf:resource="https://m82-project.org/dima-bias/ontology#Technique"/>
    <rdfs:label xml:lang="fr">biais de confusion de source</rdfs:label>
    <rdfs:label xml:lang="en">source confusion bias</rdfs:label>
    <ns1:valueCode rdf:datatype="http://www.w3.org/2001/XMLSchema#string">TE0312</ns1:valueCode>
    <rdfs:subClassOf rdf:resource="https://m82-project.org/dima-bias/ontology#MemoriseTechnique"/>
  </rdf:Description>
  <rdf:Description rdf:about="https://m82-project.org/dima-bias/ontology#SelfReference">
    <rdfs:subClassOf rdf:resource="https://m82-project.org/dima-bias/ontology#InformTactic"/>
    <rdfs:label xml:lang="fr">Auto-référence</rdfs:label>
    <rdfs:label xml:lang="en">Self-reference</rdfs:label>
    <rdf:type rdf:resource="http://www.w3.org/2002/07/owl#NamedIndividual"/>
    <rdf:type rdf:resource="https://m82-project.org/dima-bias/ontology#InformTactic"/>
    <rdf:type rdf:resource="https://m82-project.org/dima-bias/ontology#Tactic"/>
    <rdf:type rdf:resource="http://www.w3.org/2002/07/owl#Class"/>
    <rdfs:comment xml:lang="fr">Tactique qui exploite le fait que la cible pense que ses interlocuteurs partagent ses références communes.</rdfs:comment>
    <rdfs:comment xml:lang="en">A tactic based on the assumption that the audience shares the same knowledge and references.</rdfs:comment>
    <ns1:valueCode rdf:datatype="http://www.w3.org/2001/XMLSchema#string">TA0025</ns1:valueCode>
    <ns1:hasTechnique rdf:resource="https://m82-project.org/dima-bias/ontology#FalseConsensusEffect"/>
  </rdf:Description>
  <rdf:Description rdf:about="https://m82-project.org/dima-bias/ontology#BackfireEffect">
    <rdf:type rdf:resource="http://www.w3.org/2002/07/owl#Class"/>
    <rdf:type rdf:resource="http://www.w3.org/2002/07/owl#NamedIndividual"/>
    <rdf:type rdf:resource="https://m82-project.org/dima-bias/ontology#Technique"/>
    <rdf:type rdf:resource="https://m82-project.org/dima-bias/ontology#InformTechnique"/>
    <rdfs:label xml:lang="en">backfire effect</rdfs:label>
    <rdfs:label xml:lang="fr">Effet de retournement</rdfs:label>
    <rdfs:comment xml:lang="fr">Tendance à renforcer ses croyances lorsqu'on est confronté à des preuves contraires.</rdfs:comment>
    <rdfs:comment xml:lang="en">Reinforcing one’s beliefs when confronted with contradictory information.</rdfs:comment>
    <rdfs:subClassOf rdf:resource="https://m82-project.org/dima-bias/ontology#InformTechnique"/>
    <ns1:valueCode rdf:datatype="http://www.w3.org/2001/XMLSchema#string">TE0221</ns1:valueCode>
  </rdf:Description>
  <rdf:Description rdf:about="https://m82-project.org/dima-bias/ontology#9a2a4d3a26_negativitybias_3">
    <rdf:type rdf:resource="http://www.w3.org/2002/07/owl#NamedIndividual"/>
    <rdf:type rdf:resource="https://m82-project.org/dima-bias/ontology#TechniqueUsage"/>
    <ns1:hasExplanation rdf:datatype="http://www.w3.org/2001/XMLSchema#string">This argument highlights international anxiety and punitive measures, repeatedly framing Zarnia as a threat and focusing on negative consequences.</ns1:hasExplanation>
    <ns1:instantiatesTechnique rdf:resource="https://m82-project.org/dima-bias/ontology#NegativityBias"/>
  </rdf:Description>
  <rdf:Description rdf:nodeID="Nb133f359893d4ef3a9a24ec98c601c99">
    <owl:hasValue rdf:resource="https://m82-project.org/dima-bias/ontology#Act"/>
    <rdf:type rdf:resource="http://www.w3.org/2002/07/owl#Restriction"/>
    <owl:onProperty rdf:resource="https://m82-project.org/dima-bias/ontology#usesPhase"/>
  </rdf:Description>
  <rdf:Description rdf:about="https://stratcomcoe.org/influence-mini/ontology#9a2a4d3a26_conclusion_1">
    <ns1:usesTechnique rdf:resource="https://m82-project.org/dima-bias/ontology#9a2a4d3a26_negativitybias_1"/>
  </rdf:Description>
  <rdf:Description rdf:about="https://stratcomcoe.org/influence-mini/ontology#9a2a4d3a26_argument_3">
    <ns1:usesTechnique rdf:resource="https://m82-project.org/dima-bias/ontology#9a2a4d3a26_negativitybias_3"/>
  </rdf:Description>
  <rdf:Description rdf:about="https://m82-project.org/dima-bias/ontology#FalseConsensusEffect">
    <rdfs:comment xml:lang="en">Overestimating how much others share your views or behaviors.</rdfs:comment>
    <rdfs:comment xml:lang="fr">Surestimer à quel point les autres partagent nos opinions ou comportements.</rdfs:comment>
    <rdfs:label xml:lang="en">false consensus effect</rdfs:label>
    <rdfs:label xml:lang="fr">Effet de faux consensus</rdfs:label>
    <rdf:type rdf:resource="https://m82-project.org/dima-bias/ontology#InformTechnique"/>
    <rdf:type rdf:resource="http://www.w3.org/2002/07/owl#Class"/>
    <rdf:type rdf:resource="http://www.w3.org/2002/07/owl#NamedIndividual"/>
    <rdf:type rdf:resource="https://m82-project.org/dima-bias/ontology#Technique"/>
    <ns1:valueCode rdf:datatype="http://www.w3.org/2001/XMLSchema#string">TE0251</ns1:valueCode>
    <rdfs:subClassOf rdf:resource="https://m82-project.org/dima-bias/ontology#InformTechnique"/>
  </rdf:Description>
  <rdf:Description rdf:about="https://m82-project.org/dima-bias/ontology#Phase">
    <owl:disjointWith rdf:resource="https://m82-project.org/dima-bias/ontology#Technique"/>
    <owl:disjointWith rdf:resource="https://m82-project.org/dima-bias/ontology#Tactic"/>
    <rdfs:comment xml:lang="fr">L'une des quatre phases majeures du cadre DIMA : Détecter, Informer, Mémoriser, Agir.</rdfs:comment>
    <rdfs:comment xml:lang="en">One of the four major stages in the DIMA framework: Detect, Inform, Memorize, Act.</rdfs:comment>
    <rdf:type rdf:resource="http://www.w3.org/2002/07/owl#Class"/>
    <rdfs:label xml:lang="fr">Phase DIMA</rdfs:label>
    <rdfs:label xml:lang="en">DIMA Phase</rdfs:label>
  </rdf:Description>
  <rdf:Description rdf:nodeID="Ncf7c353bb1a542b2a7d0cffc91b34b12">
    <rdf:first rdf:resource="https://m82-project.org/dima-bias/ontology#isTechniqueOf"/>
    <rdf:rest rdf:resource="http://www.w3.org/1999/02/22-rdf-syntax-ns#nil"/>
  </rdf:Description>
  <rdf:Description rdf:about="https://m82-project.org/dima-bias/ontology#AvailabilityHeuristic">
    <ns1:valueCode rdf:datatype="http://www.w3.org/2001/XMLSchema#string">TE0111</ns1:valueCode>
    <rdfs:label xml:lang="en">availability heuristic</rdfs:label>
    <rdfs:label xml:lang="fr">Heuristique de disponibilité</rdfs:label>
    <rdf:type rdf:resource="http://www.w3.org/2002/07/owl#Class"/>
    <rdf:type rdf:resource="http://www.w3.org/2002/07/owl#NamedIndividual"/>
    <rdf:type rdf:resource="https://m82-project.org/dima-bias/ontology#Technique"/>
    <rdf:type rdf:resource="https://m82-project.org/dima-bias/ontology#DetectTechnique"/>
    <rdfs:comment xml:lang="en">Using readily available examples or experiences as the basis for decisions, regardless of their representativeness.</rdfs:comment>
    <rdfs:comment xml:lang="fr">Décision fondée sur des exemples ou souvenirs facilement accessibles, même s’ils ne sont pas représentatifs.</rdfs:comment>
    <rdfs:subClassOf rdf:resource="https://m82-project.org/dima-bias/ontology#DetectTechnique"/>
  </rdf:Description>
  <rdf:Description rdf:about="https://m82-project.org/dima-bias/ontology#InformArgument">
    <rdfs:label xml:lang="en">Inform argument</rdfs:label>
    <owl:equivalentClass rdf:nodeID="Nc3e48981dc3d429dbaf9af2e34de2bac"/>
    <owl:equivalentClass rdf:nodeID="N22c16a8180e64cf78cb66d45cbb94d93"/>
    <rdfs:comment xml:lang="en">Arguments that use techniques from the Inform phase.</rdfs:comment>
    <rdf:type rdf:resource="http://www.w3.org/2002/07/owl#Class"/>
  </rdf:Description>
  <rdf:Description rdf:about="https://m82-project.org/dima-bias/ontology#AnecdotalEvidenceBias">
    <rdfs:comment xml:lang="fr">Accorder plus de poids aux récits personnels qu'aux preuves statistiques.</rdfs:comment>
    <rdfs:comment xml:lang="en">Giving more weight to vivid personal stories than to statistical evidence.</rdfs:comment>
    <rdf:type rdf:resource="http://www.w3.org/2002/07/owl#Class"/>
    <rdf:type rdf:resource="http://www.w3.org/2002/07/owl#NamedIndividual"/>
    <rdf:type rdf:resource="https://m82-project.org/dima-bias/ontology#InformTechnique"/>
    <rdf:type rdf:resource="https://m82-project.org/dima-bias/ontology#Technique"/>
    <rdfs:label xml:lang="fr">Biais de la preuve anecdotique</rdfs:label>
    <rdfs:label xml:lang="en">anecdotal evidence bias</rdfs:label>
    <rdfs:subClassOf rdf:resource="https://m82-project.org/dima-bias/ontology#InformTechnique"/>
    <ns1:valueCode rdf:datatype="http://www.w3.org/2001/XMLSchema#string">TE0212</ns1:valueCode>
  </rdf:Description>
  <rdf:Description rdf:nodeID="N94876565c798488ca0503826143a59f5">
    <rdf:first rdf:resource="https://m82-project.org/dima-bias/ontology#instantiatesTechnique"/>
    <rdf:rest rdf:nodeID="Na909bfedb56543d183762981a9d8d78c"/>
  </rdf:Description>
  <rdf:Description rdf:about="https://m82-project.org/dima-bias/ontology#FadingAffectBias">
    <rdfs:label xml:lang="en">fading affect bias</rdfs:label>
    <rdfs:label xml:lang="fr">Effacement négatif</rdfs:label>
    <rdfs:comment xml:lang="fr">Les émotions négatives s'effacent plus vite que les positives dans les souvenirs.</rdfs:comment>
    <rdfs:comment xml:lang="en">Tendency to forget negative emotions faster than positive ones.</rdfs:comment>
    <rdf:type rdf:resource="https://m82-project.org/dima-bias/ontology#MemoriseTechnique"/>
    <rdf:type rdf:resource="http://www.w3.org/2002/07/owl#Class"/>
    <rdf:type rdf:resource="http://www.w3.org/2002/07/owl#NamedIndividual"/>
    <rdf:type rdf:resource="https://m82-project.org/dima-bias/ontology#Technique"/>
    <ns1:valueCode rdf:datatype="http://www.w3.org/2001/XMLSchema#string">TE0322</ns1:valueCode>
    <rdfs:subClassOf rdf:resource="https://m82-project.org/dima-bias/ontology#MemoriseTechnique"/>
  </rdf:Description>
  <rdf:Description rdf:about="https://m82-project.org/dima-bias/ontology#Memorise">
    <rdf:type rdf:resource="http://www.w3.org/2002/07/owl#Class"/>
    <rdf:type rdf:resource="http://www.w3.org/2002/07/owl#NamedIndividual"/>
    <rdf:type rdf:resource="https://m82-project.org/dima-bias/ontology#Phase"/>
    <ns1:hasTactic rdf:resource="https://m82-project.org/dima-bias/ontology#IndirectReinforcement"/>
    <ns1:hasTactic rdf:resource="https://m82-project.org/dima-bias/ontology#PreexistingReinforcement"/>
    <ns1:hasTactic rdf:resource="https://m82-project.org/dima-bias/ontology#ContentExposure"/>
    <rdfs:label xml:lang="en">MEMORISE</rdfs:label>
    <rdfs:label xml:lang="fr">MÉMORISER</rdfs:label>
    <rdfs:subClassOf rdf:resource="https://m82-project.org/dima-bias/ontology#Phase"/>
  </rdf:Description>
  <rdf:Description rdf:about="https://m82-project.org/dima-bias/ontology#isPhaseUsedBy">
    <owl:inverseOf rdf:resource="https://m82-project.org/dima-bias/ontology#usesPhase"/>
    <rdfs:label xml:lang="en">is used in argument (phase)</rdfs:label>
    <rdfs:label xml:lang="fr">est utilisée dans un argument (phase)</rdfs:label>
    <rdfs:comment xml:lang="fr">Propriété inverse inférée reliant une phase aux arguments qui l’utilisent.</rdfs:comment>
    <rdfs:comment xml:lang="en">Inverse of inferred property linking a phase to the arguments that use it.</rdfs:comment>
    <rdfs:domain rdf:resource="https://m82-project.org/dima-bias/ontology#Phase"/>
    <rdfs:range rdf:resource="https://stratcomcoe.org/influence-mini/ontology#Argument"/>
    <rdf:type rdf:resource="http://www.w3.org/2002/07/owl#ObjectProperty"/>
  </rdf:Description>
  <rdf:Description rdf:about="https://m82-project.org/dima-bias/ontology#ActTechnique">
    <rdf:type rdf:resource="http://www.w3.org/2002/07/owl#Class"/>
    <rdfs:label xml:lang="en">Act technique</rdfs:label>
    <rdfs:comment xml:lang="en">Techniques that belong to Act‑phase tactics.</rdfs:comment>
    <rdfs:subClassOf rdf:nodeID="N80520c26f6fe46da89533b0b41a7fdda"/>
    <rdfs:subClassOf rdf:resource="https://m82-project.org/dima-bias/ontology#Technique"/>
    <rdfs:subClassOf rdf:nodeID="N45cb9850dc764c98a0ca5a128d803dc9"/>
  </rdf:Description>
  <rdf:Description rdf:about="https://m82-project.org/dima-bias/ontology#DeviationFromNorm">
    <rdfs:comment xml:lang="fr">Tactique qui propose repose sur la capacité à détecter les changements dans notre environnement.</rdfs:comment>
    <rdfs:comment xml:lang="en">A tactic leveraging the detection of novelty or change in context.</rdfs:comment>
    <ns1:hasTechnique rdf:resource="https://m82-project.org/dima-bias/ontology#VonRestorffEffect"/>
    <ns1:hasTechnique rdf:resource="https://m82-project.org/dima-bias/ontology#ContrastEffect"/>
    <ns1:hasTechnique rdf:resource="https://m82-project.org/dima-bias/ontology#AnchoringBias"/>
    <rdfs:subClassOf rdf:resource="https://m82-project.org/dima-bias/ontology#DetectTactic"/>
    <rdfs:label xml:lang="en">Deviation from the norm</rdfs:label>
    <rdfs:label xml:lang="fr">Écart à la norme</rdfs:label>
    <rdf:type rdf:resource="http://www.w3.org/2002/07/owl#Class"/>
    <rdf:type rdf:resource="http://www.w3.org/2002/07/owl#NamedIndividual"/>
    <rdf:type rdf:resource="https://m82-project.org/dima-bias/ontology#DetectTactic"/>
    <rdf:type rdf:resource="https://m82-project.org/dima-bias/ontology#Tactic"/>
    <ns1:valueCode rdf:datatype="http://www.w3.org/2001/XMLSchema#string">TA0014</ns1:valueCode>
    <ns1:uuid rdf:datatype="http://www.w3.org/2001/XMLSchema#string">b7f72b4a-d8a9-4613-9d1d-f11e01e6527c</ns1:uuid>
  </rdf:Description>
  <rdf:Description rdf:about="https://m82-project.org/dima-bias/ontology">
    <dcterms:hasVersion rdf:datatype="http://www.w3.org/2001/XMLSchema#string">bf4ae6797d799fe7f0cd56e4263a209ba66c1e0c</dcterms:hasVersion>
    <dcterms:source rdf:resource="https://github.com/M82-project/DIMA/tree/bf4ae6797d799fe7f0cd56e4263a209ba66c1e0c"/>
    <rdfs:label xml:lang="fr">Ontologie des biais DIMA – Unifiée</rdfs:label>
    <rdfs:label xml:lang="en">DIMA Bias Ontology – Unified</rdfs:label>
    <owl:versionIRI rdf:resource="https://m82-project.org/dima-bias/ontology/v1.0.0"/>
    <rdf:type rdf:resource="http://www.w3.org/2002/07/owl#Ontology"/>
  </rdf:Description>
  <rdf:Description rdf:about="https://m82-project.org/dima-bias/ontology#DistinctionBias">
    <rdf:type rdf:resource="http://www.w3.org/2002/07/owl#Class"/>
    <rdf:type rdf:resource="http://www.w3.org/2002/07/owl#NamedIndividual"/>
    <rdf:type rdf:resource="https://m82-project.org/dima-bias/ontology#Technique"/>
    <rdf:type rdf:resource="https://m82-project.org/dima-bias/ontology#DetectTechnique"/>
    <rdfs:comment xml:lang="fr">Surestimer les différences entre deux options lorsqu’elles sont comparées côte à côte.</rdfs:comment>
    <rdfs:comment xml:lang="en">Tendency to overstate differences between options when evaluated simultaneously.</rdfs:comment>
    <rdfs:label xml:lang="fr">Biais de distinction</rdfs:label>
    <rdfs:label xml:lang="en">distinction bias</rdfs:label>
    <rdfs:subClassOf rdf:resource="https://m82-project.org/dima-bias/ontology#DetectTechnique"/>
    <ns1:valueCode rdf:datatype="http://www.w3.org/2001/XMLSchema#string">TE0151</ns1:valueCode>
  </rdf:Description>
  <rdf:Description rdf:about="https://m82-project.org/dima-bias/ontology#GamblersFallacy">
    <rdf:type rdf:resource="http://www.w3.org/2002/07/owl#NamedIndividual"/>
    <rdf:type rdf:resource="https://m82-project.org/dima-bias/ontology#InformTechnique"/>
    <rdf:type rdf:resource="https://m82-project.org/dima-bias/ontology#Technique"/>
    <rdf:type rdf:resource="http://www.w3.org/2002/07/owl#Class"/>
    <rdfs:label xml:lang="fr">Illusion des séries</rdfs:label>
    <rdfs:label xml:lang="en">gambler’s fallacy</rdfs:label>
    <ns1:valueCode rdf:datatype="http://www.w3.org/2001/XMLSchema#string">TE0213</ns1:valueCode>
    <rdfs:comment xml:lang="en">Believing that past random events influence future ones.</rdfs:comment>
    <rdfs:comment xml:lang="fr">Croire que les événements passés influencent la probabilité des événements futurs.</rdfs:comment>
    <rdfs:subClassOf rdf:resource="https://m82-project.org/dima-bias/ontology#InformTechnique"/>
  </rdf:Description>
  <rdf:Description rdf:about="https://m82-project.org/dima-bias/ontology#Tactic">
    <rdf:type rdf:resource="http://www.w3.org/2002/07/owl#Class"/>
    <rdfs:comment xml:lang="en">A communicative strategy used to exploit cognitive biases in narrative content.</rdfs:comment>
    <rdfs:comment xml:lang="fr">Une stratégie narrative exploitant des biais cognitifs dans un discours.</rdfs:comment>
    <rdfs:label xml:lang="en">Narrative Tactic</rdfs:label>
    <rdfs:label xml:lang="fr">Tactique narrative</rdfs:label>
    <owl:disjointWith rdf:resource="https://m82-project.org/dima-bias/ontology#Technique"/>
  </rdf:Description>
  <rdf:Description rdf:about="https://m82-project.org/dima-bias/ontology#SuggestionEffect">
    <rdf:type rdf:resource="http://www.w3.org/2002/07/owl#Class"/>
    <rdf:type rdf:resource="http://www.w3.org/2002/07/owl#NamedIndividual"/>
    <rdf:type rdf:resource="https://m82-project.org/dima-bias/ontology#Technique"/>
    <rdf:type rdf:resource="https://m82-project.org/dima-bias/ontology#MemoriseTechnique"/>
    <rdfs:subClassOf rdf:resource="https://m82-project.org/dima-bias/ontology#MemoriseTechnique"/>
    <rdfs:label xml:lang="fr">Effet de suggestion</rdfs:label>
    <rdfs:label xml:lang="en">suggestion effect</rdfs:label>
    <rdfs:comment xml:lang="en">The tendency for suggestions to influence memory construction.</rdfs:comment>
    <rdfs:comment xml:lang="fr">Tendance à altérer ou créer des souvenirs sous l'effet de suggestions extérieures.</rdfs:comment>
    <ns1:valueCode rdf:datatype="http://www.w3.org/2001/XMLSchema#string">TE0314</ns1:valueCode>
  </rdf:Description>
  <rdf:Description rdf:about="https://m82-project.org/dima-bias/ontology#OmissionBias">
    <rdf:type rdf:resource="http://www.w3.org/2002/07/owl#Class"/>
    <rdf:type rdf:resource="http://www.w3.org/2002/07/owl#NamedIndividual"/>
    <rdf:type rdf:resource="https://m82-project.org/dima-bias/ontology#Technique"/>
    <rdf:type rdf:resource="https://m82-project.org/dima-bias/ontology#ActTechnique"/>
    <rdfs:label xml:lang="en">omission bias</rdfs:label>
    <rdfs:label xml:lang="fr">Biais d'omission</rdfs:label>
    <rdfs:comment xml:lang="fr">Considérer qu'un tort causé par inaction est moins grave qu’un tort causé par action.</rdfs:comment>
    <rdfs:comment xml:lang="en">Preferring inaction over action even when it leads to worse outcomes.</rdfs:comment>
    <rdfs:subClassOf rdf:resource="https://m82-project.org/dima-bias/ontology#ActTechnique"/>
    <ns1:valueCode rdf:datatype="http://www.w3.org/2001/XMLSchema#string">TE0431</ns1:valueCode>
  </rdf:Description>
  <rdf:Description rdf:about="https://m82-project.org/dima-bias/ontology#c9ce7d9bb7_vonrestorffeffect_4">
    <ns1:instantiatesTechnique rdf:resource="https://m82-project.org/dima-bias/ontology#VonRestorffEffect"/>
    <rdf:type rdf:resource="http://www.w3.org/2002/07/owl#NamedIndividual"/>
    <rdf:type rdf:resource="https://m82-project.org/dima-bias/ontology#TechniqueUsage"/>
    <ns1:hasExplanation rdf:datatype="http://www.w3.org/2001/XMLSchema#string">The development isolates the action of the 'international community' as a distinct, memorable shift, setting it apart from the more routine actions of regional powers and the Security Council, thus exploiting the Von Restorff Effect.</ns1:hasExplanation>
  </rdf:Description>
  <rdf:Description rdf:nodeID="N86841e2330bc451a9c93dd8c59b7106c">
    <owl:intersectionOf rdf:nodeID="N89ff6e16b09b492a82374fce32449caa"/>
    <rdf:type rdf:resource="http://www.w3.org/2002/07/owl#Class"/>
  </rdf:Description>
  <rdf:Description rdf:about="https://m82-project.org/dima-bias/ontology#NegativityBias">
    <ns1:valueCode rdf:datatype="http://www.w3.org/2001/XMLSchema#string">TE0132</ns1:valueCode>
    <rdfs:comment xml:lang="fr">Accorder plus d’attention et de poids aux expériences négatives qu’aux positives.</rdfs:comment>
    <rdfs:comment xml:lang="en">Giving more attention and weight to negative experiences over positive ones.</rdfs:comment>
    <rdf:type rdf:resource="http://www.w3.org/2002/07/owl#Class"/>
    <rdf:type rdf:resource="https://m82-project.org/dima-bias/ontology#DetectTechnique"/>
    <rdf:type rdf:resource="http://www.w3.org/2002/07/owl#NamedIndividual"/>
    <rdf:type rdf:resource="https://m82-project.org/dima-bias/ontology#Technique"/>
    <rdfs:label xml:lang="fr">Biais de négativité</rdfs:label>
    <rdfs:label xml:lang="en">negativity bias</rdfs:label>
    <rdfs:subClassOf rdf:resource="https://m82-project.org/dima-bias/ontology#DetectTechnique"/>
  </rdf:Description>
  <rdf:Description rdf:about="https://stratcomcoe.org/influence-mini/ontology#c9ce7d9bb7_premise_2">
    <ns1:usesTechnique rdf:resource="https://m82-project.org/dima-bias/ontology#c9ce7d9bb7_negativitybias_1"/>
  </rdf:Description>
  <rdf:Description rdf:nodeID="Nca1fd162941d4763a4745646f49a2841">
    <owl:onProperty rdf:resource="https://m82-project.org/dima-bias/ontology#usesPhase"/>
    <owl:hasValue rdf:resource="https://m82-project.org/dima-bias/ontology#Inform"/>
    <rdf:type rdf:resource="http://www.w3.org/2002/07/owl#Restriction"/>
  </rdf:Description>
  <rdf:Description rdf:about="https://m82-project.org/dima-bias/ontology#GeneralizationAndStereotypes">
    <rdf:type rdf:resource="http://www.w3.org/2002/07/owl#Class"/>
    <rdf:type rdf:resource="http://www.w3.org/2002/07/owl#NamedIndividual"/>
    <rdf:type rdf:resource="https://m82-project.org/dima-bias/ontology#Tactic"/>
    <rdf:type rdf:resource="https://m82-project.org/dima-bias/ontology#InformTactic"/>
    <rdfs:subClassOf rdf:resource="https://m82-project.org/dima-bias/ontology#InformTactic"/>
    <rdfs:label xml:lang="en">Generalization and reinforcement of stereotypes</rdfs:label>
    <rdfs:label xml:lang="fr">Généralisation et renforcement de stéréotypes</rdfs:label>
    <rdfs:comment xml:lang="en">A tactic aiming to simplify perceived information to make it more acceptable or understandable to the target.</rdfs:comment>
    <rdfs:comment xml:lang="fr">Tactique qui vise à simplifier une ou des informations perçues pour les rendre acceptables et/ou intelligibles par la cible.</rdfs:comment>
    <ns1:hasTechnique rdf:resource="https://m82-project.org/dima-bias/ontology#BackfireEffect"/>
    <ns1:valueCode rdf:datatype="http://www.w3.org/2001/XMLSchema#string">TA0022</ns1:valueCode>
  </rdf:Description>
  <rdf:Description rdf:about="https://m82-project.org/dima-bias/ontology#usesTactic">
    <rdfs:label xml:lang="fr">utilise une tactique</rdfs:label>
    <rdfs:label xml:lang="en">uses tactic</rdfs:label>
    <rdfs:comment xml:lang="en">Inferred property: links an argument to a tactic via the technique it uses.</rdfs:comment>
    <rdfs:comment xml:lang="fr">Propriété inférée : associe un argument à une tactique via la technique utilisée.</rdfs:comment>
    <rdf:type rdf:resource="http://www.w3.org/2002/07/owl#ObjectProperty"/>
    <rdfs:range rdf:resource="https://m82-project.org/dima-bias/ontology#Tactic"/>
    <rdfs:domain rdf:resource="https://stratcomcoe.org/influence-mini/ontology#Argument"/>
  </rdf:Description>
  <rdf:Description rdf:about="https://m82-project.org/dima-bias/ontology#Detect">
    <rdf:type rdf:resource="http://www.w3.org/2002/07/owl#Class"/>
    <rdf:type rdf:resource="http://www.w3.org/2002/07/owl#NamedIndividual"/>
    <rdf:type rdf:resource="https://m82-project.org/dima-bias/ontology#Phase"/>
    <ns1:hasTactic rdf:resource="https://m82-project.org/dima-bias/ontology#SignificantDetail"/>
    <ns1:hasTactic rdf:resource="https://m82-project.org/dima-bias/ontology#PreExistingInformation"/>
    <ns1:hasTactic rdf:resource="https://m82-project.org/dima-bias/ontology#DivisiveInformation"/>
    <ns1:hasTactic rdf:resource="https://m82-project.org/dima-bias/ontology#DeviationFromNorm"/>
    <ns1:hasTactic rdf:resource="https://m82-project.org/dima-bias/ontology#RepeatedExposureInformation"/>
    <rdfs:label xml:lang="en">DETECT</rdfs:label>
    <rdfs:label xml:lang="fr">DÉTECTER</rdfs:label>
    <rdfs:subClassOf rdf:resource="https://m82-project.org/dima-bias/ontology#Phase"/>
  </rdf:Description>
  <rdf:Description rdf:about="https://m82-project.org/dima-bias/ontology#InformTactic">
    <rdfs:label xml:lang="en">Inform tactic</rdfs:label>
    <rdfs:comment xml:lang="en">Tactics associated with the Inform phase.</rdfs:comment>
    <rdf:type rdf:resource="http://www.w3.org/2002/07/owl#Class"/>
    <rdfs:subClassOf rdf:nodeID="Nc44f1fe74c6547d1b7a02e1fd09e3b03"/>
    <rdfs:subClassOf rdf:resource="https://m82-project.org/dima-bias/ontology#Tactic"/>
    <rdfs:subClassOf rdf:nodeID="Ne4e356813f2144a68e4c738cefba274c"/>
  </rdf:Description>
  <rdf:Description rdf:about="https://m82-project.org/dima-bias/ontology#PreexistingReinforcement">
    <rdfs:label xml:lang="en">Pre-existing reinforcement</rdfs:label>
    <rdfs:label xml:lang="fr">Renforcement pré-existant</rdfs:label>
    <ns1:hasTechnique rdf:resource="https://m82-project.org/dima-bias/ontology#FadingAffectBias"/>
    <ns1:hasTechnique rdf:resource="https://m82-project.org/dima-bias/ontology#ImplicitStereotype"/>
    <ns1:hasTechnique rdf:resource="https://m82-project.org/dima-bias/ontology#ContextEffect_Memorise"/>
    <rdf:type rdf:resource="https://m82-project.org/dima-bias/ontology#MemoriseTactic"/>
    <rdf:type rdf:resource="https://m82-project.org/dima-bias/ontology#Tactic"/>
    <rdf:type rdf:resource="http://www.w3.org/2002/07/owl#Class"/>
    <rdf:type rdf:resource="http://www.w3.org/2002/07/owl#NamedIndividual"/>
    <rdfs:comment xml:lang="fr">Tactique qui favorise la mémorisation d'une information en s'appuyant sur des stéréotypes ou des croyances pré-existantes.</rdfs:comment>
    <rdfs:comment xml:lang="en">A tactic that helps memorize information by leveraging stereotypes or pre-existing beliefs.</rdfs:comment>
    <rdfs:subClassOf rdf:resource="https://m82-project.org/dima-bias/ontology#MemoriseTactic"/>
    <ns1:valueCode rdf:datatype="http://www.w3.org/2001/XMLSchema#string">TA0032</ns1:valueCode>
  </rdf:Description>
  <rdf:Description rdf:about="https://m82-project.org/dima-bias/ontology#ContextEffect">
    <rdf:type rdf:resource="http://www.w3.org/2002/07/owl#Class"/>
    <rdf:type rdf:resource="http://www.w3.org/2002/07/owl#NamedIndividual"/>
    <rdf:type rdf:resource="https://m82-project.org/dima-bias/ontology#Technique"/>
    <rdf:type rdf:resource="https://m82-project.org/dima-bias/ontology#DetectTechnique"/>
    <rdfs:subClassOf rdf:resource="https://m82-project.org/dima-bias/ontology#DetectTechnique"/>
    <rdfs:label xml:lang="en">context effect</rdfs:label>
    <rdfs:label xml:lang="fr">Effet de contexte</rdfs:label>
    <rdfs:comment xml:lang="fr">Analyser une perception par rapport à des situations proches ou similaires.</rdfs:comment>
    <rdfs:comment xml:lang="en">Tendency to interpret perceptions in relation to nearby or similar situations.</rdfs:comment>
    <ns1:valueCode rdf:datatype="http://www.w3.org/2001/XMLSchema#string">TE0122</ns1:valueCode>
  </rdf:Description>
  <rdf:Description rdf:about="https://stratcomcoe.org/influence-mini/ontology#c9ce7d9bb7_argument_0">
    <ns1:usesTechnique rdf:resource="https://m82-project.org/dima-bias/ontology#c9ce7d9bb7_vonrestorffeffect_0"/>
  </rdf:Description>
  <rdf:Description rdf:about="https://m82-project.org/dima-bias/ontology#SignificantDetail">
    <rdf:type rdf:resource="https://m82-project.org/dima-bias/ontology#Tactic"/>
    <rdf:type rdf:resource="http://www.w3.org/2002/07/owl#Class"/>
    <rdf:type rdf:resource="http://www.w3.org/2002/07/owl#NamedIndividual"/>
    <rdf:type rdf:resource="https://m82-project.org/dima-bias/ontology#DetectTactic"/>
    <rdfs:comment xml:lang="en">A tactic exploiting the human tendency to focus on isolated details and attribute meaning to them.</rdfs:comment>
    <rdfs:comment xml:lang="fr">Tactique qui exploite la propension d'une cible à détecter un détail et à lui donner du sens.</rdfs:comment>
    <ns1:uuid rdf:datatype="http://www.w3.org/2001/XMLSchema#string">e8d27437-6c1d-4e07-9f33-d8e164bb9d2e</ns1:uuid>
    <ns1:hasTechnique rdf:resource="https://m82-project.org/dima-bias/ontology#DistinctionBias"/>
    <ns1:hasTechnique rdf:resource="https://m82-project.org/dima-bias/ontology#WeberFechnerLaw"/>
    <ns1:valueCode rdf:datatype="http://www.w3.org/2001/XMLSchema#string">TA0015</ns1:valueCode>
    <rdfs:subClassOf rdf:resource="https://m82-project.org/dima-bias/ontology#DetectTactic"/>
    <rdfs:label xml:lang="en">Significant detail</rdfs:label>
    <rdfs:label xml:lang="fr">Détail signifiant</rdfs:label>
  </rdf:Description>
  <rdf:Description rdf:about="https://m82-project.org/dima-bias/ontology#HomogeneityBias">
    <ns1:valueCode rdf:datatype="http://www.w3.org/2001/XMLSchema#string">TE0231</ns1:valueCode>
    <rdfs:comment xml:lang="fr">Tendance à voir les membres d’un groupe externe comme homogènes.</rdfs:comment>
    <rdfs:comment xml:lang="en">Perceiving members of an out-group as more similar than they really are.</rdfs:comment>
    <rdfs:label xml:lang="en">homogeneity bias</rdfs:label>
    <rdfs:label xml:lang="fr">Biais d'homogénéité</rdfs:label>
    <rdf:type rdf:resource="https://m82-project.org/dima-bias/ontology#InformTechnique"/>
    <rdf:type rdf:resource="http://www.w3.org/2002/07/owl#Class"/>
    <rdf:type rdf:resource="http://www.w3.org/2002/07/owl#NamedIndividual"/>
    <rdf:type rdf:resource="https://m82-project.org/dima-bias/ontology#Technique"/>
    <rdfs:subClassOf rdf:resource="https://m82-project.org/dima-bias/ontology#InformTechnique"/>
  </rdf:Description>
  <rdf:Description rdf:about="https://m82-project.org/dima-bias/ontology#AuthorityBias">
    <ns1:valueCode rdf:datatype="http://www.w3.org/2001/XMLSchema#string">TE0422</ns1:valueCode>
    <rdfs:comment xml:lang="fr">Tendance à accorder plus de crédibilité ou à suivre les directives de figures d’autorité.</rdfs:comment>
    <rdfs:comment xml:lang="en">Tendency to follow directives or believe information from perceived authorities.</rdfs:comment>
    <rdf:type rdf:resource="http://www.w3.org/2002/07/owl#NamedIndividual"/>
    <rdf:type rdf:resource="https://m82-project.org/dima-bias/ontology#Technique"/>
    <rdf:type rdf:resource="https://m82-project.org/dima-bias/ontology#ActTechnique"/>
    <rdf:type rdf:resource="http://www.w3.org/2002/07/owl#Class"/>
    <rdfs:label xml:lang="fr">biais d'autorité</rdfs:label>
    <rdfs:label xml:lang="en">authority bias</rdfs:label>
    <rdfs:subClassOf rdf:resource="https://m82-project.org/dima-bias/ontology#ActTechnique"/>
  </rdf:Description>
  <rdf:Description rdf:about="https://m82-project.org/dima-bias/ontology#RepeatedExposureInformation">
    <rdfs:comment xml:lang="fr">Tactique qui repose sur l’exploitation de la répétition de l’information en vue de faciliter sa détection par la cible.</rdfs:comment>
    <rdfs:comment xml:lang="en">A tactic based on exploiting repetition to improve information detection.</rdfs:comment>
    <rdf:type rdf:resource="https://m82-project.org/dima-bias/ontology#DetectTactic"/>
    <rdf:type rdf:resource="https://m82-project.org/dima-bias/ontology#Tactic"/>
    <rdf:type rdf:resource="http://www.w3.org/2002/07/owl#Class"/>
    <rdf:type rdf:resource="http://www.w3.org/2002/07/owl#NamedIndividual"/>
    <ns1:uuid rdf:datatype="http://www.w3.org/2001/XMLSchema#string">a2d9c63d-f4d6-4183-b0f7-2169b8c2d8d4</ns1:uuid>
    <rdfs:label xml:lang="fr">Information à exposition répétée</rdfs:label>
    <rdfs:label xml:lang="en">Repeated exposure information</rdfs:label>
    <rdfs:subClassOf rdf:resource="https://m82-project.org/dima-bias/ontology#DetectTactic"/>
    <ns1:hasTechnique rdf:resource="https://m82-project.org/dima-bias/ontology#FrequencyIllusion"/>
    <ns1:hasTechnique rdf:resource="https://m82-project.org/dima-bias/ontology#ContextEffect"/>
    <ns1:valueCode rdf:datatype="http://www.w3.org/2001/XMLSchema#string">TA0012</ns1:valueCode>
  </rdf:Description>
  <rdf:Description rdf:nodeID="N1029932e0a2f49df875a9ee49ab55619">
    <owl:intersectionOf rdf:nodeID="Na136a50d2c1842e3bb5aef3422227dfe"/>
    <rdf:type rdf:resource="http://www.w3.org/2002/07/owl#Class"/>
  </rdf:Description>
  <rdf:Description rdf:about="https://m82-project.org/dima-bias/ontology#ContrastEffect">
    <rdfs:label xml:lang="fr">Effet de contraste</rdfs:label>
    <rdfs:label xml:lang="en">contrast effect</rdfs:label>
    <ns1:valueCode rdf:datatype="http://www.w3.org/2001/XMLSchema#string">TE0143</ns1:valueCode>
    <rdfs:comment xml:lang="fr">Modification de la perception par comparaison avec un autre élément observé auparavant.</rdfs:comment>
    <rdfs:comment xml:lang="en">Perception of an item is influenced by comparison with what came before.</rdfs:comment>
    <rdf:type rdf:resource="http://www.w3.org/2002/07/owl#Class"/>
    <rdf:type rdf:resource="https://m82-project.org/dima-bias/ontology#DetectTechnique"/>
    <rdf:type rdf:resource="http://www.w3.org/2002/07/owl#NamedIndividual"/>
    <rdf:type rdf:resource="https://m82-project.org/dima-bias/ontology#Technique"/>
    <rdfs:subClassOf rdf:resource="https://m82-project.org/dima-bias/ontology#DetectTechnique"/>
  </rdf:Description>
  <rdf:Description rdf:about="https://m82-project.org/dima-bias/ontology#PreExistingInformation">
    <rdf:type rdf:resource="http://www.w3.org/2002/07/owl#NamedIndividual"/>
    <rdf:type rdf:resource="https://m82-project.org/dima-bias/ontology#DetectTactic"/>
    <rdf:type rdf:resource="https://m82-project.org/dima-bias/ontology#Tactic"/>
    <rdf:type rdf:resource="http://www.w3.org/2002/07/owl#Class"/>
    <rdfs:comment xml:lang="fr">Tactique qui utilise des informations préexistantes ou des croyances établies pour capter l’attention de la cible.</rdfs:comment>
    <rdfs:comment xml:lang="en">A tactic that uses pre-existing beliefs or knowledge to attract attention.</rdfs:comment>
    <ns1:hasTechnique rdf:resource="https://m82-project.org/dima-bias/ontology#MereExposureEffect"/>
    <ns1:hasTechnique rdf:resource="https://m82-project.org/dima-bias/ontology#AvailabilityHeuristic"/>
    <ns1:valueCode rdf:datatype="http://www.w3.org/2001/XMLSchema#string">TA0011</ns1:valueCode>
    <rdfs:subClassOf rdf:resource="https://m82-project.org/dima-bias/ontology#DetectTactic"/>
    <rdfs:label xml:lang="en">Pre-existing information</rdfs:label>
    <rdfs:label xml:lang="fr">Information préexistante</rdfs:label>
    <ns1:uuid rdf:datatype="http://www.w3.org/2001/XMLSchema#string">f7b94d9e-2e5b-4082-9f96-ab704e6e1d95</ns1:uuid>
  </rdf:Description>
  <rdf:Description rdf:about="https://m82-project.org/dima-bias/ontology#valueCode">
    <rdf:type rdf:resource="http://www.w3.org/2002/07/owl#AnnotationProperty"/>
    <rdfs:comment xml:lang="fr">Code de la taxonomie source (ex. : TA0011, TE0111).</rdfs:comment>
    <rdfs:comment xml:lang="en">Code from the source taxonomy (e.g., TA0011, TE0111).</rdfs:comment>
    <rdfs:label xml:lang="en">Value code</rdfs:label>
    <rdfs:label xml:lang="fr">Code de valeur</rdfs:label>
  </rdf:Description>
  <rdf:Description rdf:about="https://m82-project.org/dima-bias/ontology#RecencyEffect">
    <rdfs:label xml:lang="en">recency effect</rdfs:label>
    <rdfs:label xml:lang="fr">Effet de récence</rdfs:label>
    <rdfs:comment xml:lang="en">Most recent information is remembered better.</rdfs:comment>
    <rdfs:comment xml:lang="fr">Les informations les plus récentes influencent davantage la mémoire et les décisions.</rdfs:comment>
    <rdf:type rdf:resource="http://www.w3.org/2002/07/owl#Class"/>
    <rdf:type rdf:resource="http://www.w3.org/2002/07/owl#NamedIndividual"/>
    <rdf:type rdf:resource="https://m82-project.org/dima-bias/ontology#Technique"/>
    <rdf:type rdf:resource="https://m82-project.org/dima-bias/ontology#MemoriseTechnique"/>
    <rdfs:subClassOf rdf:resource="https://m82-project.org/dima-bias/ontology#MemoriseTechnique"/>
    <ns1:valueCode rdf:datatype="http://www.w3.org/2001/XMLSchema#string">TE0331</ns1:valueCode>
  </rdf:Description>
  <rdf:Description rdf:about="https://m82-project.org/dima-bias/ontology#c9ce7d9bb7_negativitybias_2">
    <ns1:hasExplanation rdf:datatype="http://www.w3.org/2001/XMLSchema#string">The conclusion frames the situation as one where Caldria is subjected to 'deliberate intimidation,' emphasizing threat and negative intent, thus exploiting negativity bias.</ns1:hasExplanation>
    <ns1:instantiatesTechnique rdf:resource="https://m82-project.org/dima-bias/ontology#NegativityBias"/>
    <rdf:type rdf:resource="http://www.w3.org/2002/07/owl#NamedIndividual"/>
    <rdf:type rdf:resource="https://m82-project.org/dima-bias/ontology#TechniqueUsage"/>
  </rdf:Description>
  <rdf:Description rdf:about="https://m82-project.org/dima-bias/ontology#IllusoryCorrelationBias">
    <ns1:valueCode rdf:datatype="http://www.w3.org/2001/XMLSchema#string">TE0211</ns1:valueCode>
    <rdfs:label xml:lang="fr">Biais de corrélation illusoire</rdfs:label>
    <rdfs:label xml:lang="en">illusory correlation bias</rdfs:label>
    <rdf:type rdf:resource="http://www.w3.org/2002/07/owl#Class"/>
    <rdf:type rdf:resource="http://www.w3.org/2002/07/owl#NamedIndividual"/>
    <rdf:type rdf:resource="https://m82-project.org/dima-bias/ontology#InformTechnique"/>
    <rdf:type rdf:resource="https://m82-project.org/dima-bias/ontology#Technique"/>
    <rdfs:comment xml:lang="en">Perceiving a false link between unrelated events or data.</rdfs:comment>
    <rdfs:comment xml:lang="fr">Tendance à percevoir un lien entre des événements ou des éléments non corrélés.</rdfs:comment>
    <rdfs:subClassOf rdf:resource="https://m82-project.org/dima-bias/ontology#InformTechnique"/>
  </rdf:Description>
  <rdf:Description rdf:about="https://m82-project.org/dima-bias/ontology#OzaekomiWaza">
    <rdfs:comment xml:lang="en">A tactic that induces passivity or decision paralysis in the target.</rdfs:comment>
    <rdfs:comment xml:lang="fr">Tactique qui consiste à favoriser chez une cible, l'immobilisme et l'absence d'action.</rdfs:comment>
    <ns1:hasTechnique rdf:resource="https://m82-project.org/dima-bias/ontology#OmissionBias"/>
    <ns1:hasTechnique rdf:resource="https://m82-project.org/dima-bias/ontology#InformationOverload"/>
    <ns1:hasTechnique rdf:resource="https://m82-project.org/dima-bias/ontology#StatusQuoBias"/>
    <ns1:valueCode rdf:datatype="http://www.w3.org/2001/XMLSchema#string">TA0043</ns1:valueCode>
    <rdfs:subClassOf rdf:resource="https://m82-project.org/dima-bias/ontology#ActTactic"/>
    <rdf:type rdf:resource="https://m82-project.org/dima-bias/ontology#Tactic"/>
    <rdf:type rdf:resource="http://www.w3.org/2002/07/owl#Class"/>
    <rdf:type rdf:resource="http://www.w3.org/2002/07/owl#NamedIndividual"/>
    <rdf:type rdf:resource="https://m82-project.org/dima-bias/ontology#ActTactic"/>
    <rdfs:label xml:lang="en">Ozaekomi waza (immobilization control)</rdfs:label>
    <rdfs:label xml:lang="fr">Ozaekomi waza (contrôle par immobilisation)</rdfs:label>
  </rdf:Description>
  <rdf:Description rdf:about="https://m82-project.org/dima-bias/ontology#DetectArgument">
    <rdfs:label xml:lang="en">Detect argument</rdfs:label>
    <rdfs:comment xml:lang="en">Arguments that use techniques from the Detect phase.</rdfs:comment>
    <owl:equivalentClass rdf:nodeID="N86841e2330bc451a9c93dd8c59b7106c"/>
    <owl:equivalentClass rdf:nodeID="N944ff1df99794d228a1fce9758f78edf"/>
    <rdf:type rdf:resource="http://www.w3.org/2002/07/owl#Class"/>
  </rdf:Description>
  <rdf:Description rdf:nodeID="N5e3f3ec777cf49208d0c8ed8d42495dd">
    <owl:onProperty rdf:resource="https://m82-project.org/dima-bias/ontology#usesPhase"/>
    <owl:hasValue rdf:resource="https://m82-project.org/dima-bias/ontology#Inform"/>
    <rdf:type rdf:resource="http://www.w3.org/2002/07/owl#Restriction"/>
  </rdf:Description>
  <rdf:Description rdf:about="https://m82-project.org/dima-bias/ontology#DivisiveInformation">
    <rdfs:subClassOf rdf:resource="https://m82-project.org/dima-bias/ontology#DetectTactic"/>
    <ns1:hasTechnique rdf:resource="https://m82-project.org/dima-bias/ontology#NegativityBias"/>
    <ns1:hasTechnique rdf:resource="https://m82-project.org/dima-bias/ontology#BizarrenessEffect"/>
    <ns1:valueCode rdf:datatype="http://www.w3.org/2001/XMLSchema#string">TA0013</ns1:valueCode>
    <rdfs:label xml:lang="fr">Information clivante</rdfs:label>
    <rdfs:label xml:lang="en">Divisive information</rdfs:label>
    <rdf:type rdf:resource="http://www.w3.org/2002/07/owl#Class"/>
    <rdf:type rdf:resource="http://www.w3.org/2002/07/owl#NamedIndividual"/>
    <rdf:type rdf:resource="https://m82-project.org/dima-bias/ontology#DetectTactic"/>
    <rdf:type rdf:resource="https://m82-project.org/dima-bias/ontology#Tactic"/>
    <rdfs:comment xml:lang="en">A tactic that highlights strange, controversial or surprising content to attract attention.</rdfs:comment>
    <rdfs:comment xml:lang="fr">Tactique qui favorise les informations clivantes, étranges ou surprenantes pour capter l’attention de la cible.</rdfs:comment>
    <ns1:uuid rdf:datatype="http://www.w3.org/2001/XMLSchema#string">d8f6b6c4-e9b1-4c16-9d8c-2b3ce6d2f332</ns1:uuid>
  </rdf:Description>
  <rdf:Description rdf:about="https://m82-project.org/dima-bias/ontology#ImplicitStereotype">
    <rdfs:label xml:lang="en">implicit stereotype</rdfs:label>
    <rdfs:label xml:lang="fr">Stéréotype implicite</rdfs:label>
    <rdf:type rdf:resource="http://www.w3.org/2002/07/owl#NamedIndividual"/>
    <rdf:type rdf:resource="https://m82-project.org/dima-bias/ontology#MemoriseTechnique"/>
    <rdf:type rdf:resource="http://www.w3.org/2002/07/owl#Class"/>
    <rdf:type rdf:resource="https://m82-project.org/dima-bias/ontology#Technique"/>
    <ns1:valueCode rdf:datatype="http://www.w3.org/2001/XMLSchema#string">TE0321</ns1:valueCode>
    <rdfs:comment xml:lang="en">Stereotypes that influence judgment or memory unconsciously.</rdfs:comment>
    <rdfs:comment xml:lang="fr">Stéréotypes influençant inconsciemment la mémoire ou le jugement.</rdfs:comment>
    <rdfs:subClassOf rdf:resource="https://m82-project.org/dima-bias/ontology#MemoriseTechnique"/>
  </rdf:Description>
  <rdf:Description rdf:nodeID="Nbbbfe1fd0a7141f1b544222281476f4d">
    <rdf:rest rdf:resource="http://www.w3.org/1999/02/22-rdf-syntax-ns#nil"/>
    <rdf:first rdf:nodeID="N2292c5effbe645e49efbaefd7a3f526f"/>
  </rdf:Description>
  <rdf:Description rdf:about="https://m82-project.org/dima-bias/ontology#Inform">
    <rdfs:label xml:lang="en">INFORM</rdfs:label>
    <rdfs:label xml:lang="fr">INFORMER</rdfs:label>
    <rdf:type rdf:resource="https://m82-project.org/dima-bias/ontology#Phase"/>
    <rdf:type rdf:resource="http://www.w3.org/2002/07/owl#Class"/>
    <rdf:type rdf:resource="http://www.w3.org/2002/07/owl#NamedIndividual"/>
    <ns1:hasTactic rdf:resource="https://m82-project.org/dima-bias/ontology#FamiliaritySuperiority"/>
    <ns1:hasTactic rdf:resource="https://m82-project.org/dima-bias/ontology#TemporalProjection"/>
    <ns1:hasTactic rdf:resource="https://m82-project.org/dima-bias/ontology#GeneralizationAndStereotypes"/>
    <ns1:hasTactic rdf:resource="https://m82-project.org/dima-bias/ontology#SelfReference"/>
    <ns1:hasTactic rdf:resource="https://m82-project.org/dima-bias/ontology#PatternCreation"/>
    <ns1:hasTactic rdf:resource="https://m82-project.org/dima-bias/ontology#Simplification"/>
    <rdfs:subClassOf rdf:resource="https://m82-project.org/dima-bias/ontology#Phase"/>
  </rdf:Description>
  <rdf:Description rdf:about="https://m82-project.org/dima-bias/ontology#IndirectReinforcement">
    <rdf:type rdf:resource="https://m82-project.org/dima-bias/ontology#Tactic"/>
    <rdf:type rdf:resource="http://www.w3.org/2002/07/owl#Class"/>
    <rdf:type rdf:resource="http://www.w3.org/2002/07/owl#NamedIndividual"/>
    <rdf:type rdf:resource="https://m82-project.org/dima-bias/ontology#MemoriseTactic"/>
    <ns1:valueCode rdf:datatype="http://www.w3.org/2001/XMLSchema#string">TA0031</ns1:valueCode>
    <rdfs:label xml:lang="fr">Renforcement indirect</rdfs:label>
    <rdfs:label xml:lang="en">Indirect reinforcement</rdfs:label>
    <rdfs:comment xml:lang="fr">Tactique qui favorise la mémorisation et la construction de souvenirs par renforcement de sources secondaires.</rdfs:comment>
    <rdfs:comment xml:lang="en">A tactic that supports memory formation by reinforcing secondary sources.</rdfs:comment>
    <ns1:hasTechnique rdf:resource="https://m82-project.org/dima-bias/ontology#SuggestionEffect"/>
    <ns1:hasTechnique rdf:resource="https://m82-project.org/dima-bias/ontology#SourceConfusionBias"/>
    <ns1:hasTechnique rdf:resource="https://m82-project.org/dima-bias/ontology#SpacingEffect"/>
    <rdfs:subClassOf rdf:resource="https://m82-project.org/dima-bias/ontology#MemoriseTactic"/>
  </rdf:Description>
  <rdf:Description rdf:about="https://m82-project.org/dima-bias/ontology#c9ce7d9bb7_vonrestorffeffect_1">
    <ns1:instantiatesTechnique rdf:resource="https://m82-project.org/dima-bias/ontology#VonRestorffEffect"/>
    <rdf:type rdf:resource="https://m82-project.org/dima-bias/ontology#TechniqueUsage"/>
    <rdf:type rdf:resource="http://www.w3.org/2002/07/owl#NamedIndividual"/>
    <ns1:hasExplanation rdf:datatype="http://www.w3.org/2001/XMLSchema#string">The argument isolates the warning from 'independent experts' as a distinct and memorable element, contrasting it with the official Velmoran stance and drawing special attention to this perspective.</ns1:hasExplanation>
  </rdf:Description>
  <rdf:Description rdf:nodeID="N4a19cd0027da40b390e35a83c62e1ccc">
    <rdf:rest rdf:nodeID="Nb837f70aaca6452d8df14d0559ef0ec0"/>
    <rdf:first rdf:resource="https://stratcomcoe.org/influence-mini/ontology#Argument"/>
  </rdf:Description>
  <rdf:Description rdf:about="https://m82-project.org/dima-bias/ontology#Technique">
    <rdfs:label xml:lang="fr">Technique cognitive</rdfs:label>
    <rdfs:label xml:lang="en">Cognitive Technique</rdfs:label>
    <rdfs:comment xml:lang="en">A cognitive bias or psychological mechanism leveraged by a tactic.</rdfs:comment>
    <rdfs:comment xml:lang="fr">Un biais cognitif ou mécanisme psychologique utilisé dans une tactique.</rdfs:comment>
    <rdf:type rdf:resource="http://www.w3.org/2002/07/owl#Class"/>
  </rdf:Description>
  <rdf:Description rdf:about="https://m82-project.org/dima-bias/ontology#PatternCreation">
    <ns1:hasTechnique rdf:resource="https://m82-project.org/dima-bias/ontology#GamblersFallacy"/>
    <ns1:hasTechnique rdf:resource="https://m82-project.org/dima-bias/ontology#IllusoryCorrelationBias"/>
    <ns1:hasTechnique rdf:resource="https://m82-project.org/dima-bias/ontology#AnecdotalEvidenceBias"/>
    <rdfs:comment xml:lang="fr">Tactique qui permet de mettre en récit une information reçue, de l’intégrer dans un contexte préexistant.</rdfs:comment>
    <rdfs:comment xml:lang="en">A tactic that integrates received information into an existing narrative.</rdfs:comment>
    <rdf:type rdf:resource="https://m82-project.org/dima-bias/ontology#Tactic"/>
    <rdf:type rdf:resource="https://m82-project.org/dima-bias/ontology#InformTactic"/>
    <rdf:type rdf:resource="http://www.w3.org/2002/07/owl#Class"/>
    <rdf:type rdf:resource="http://www.w3.org/2002/07/owl#NamedIndividual"/>
    <ns1:valueCode rdf:datatype="http://www.w3.org/2001/XMLSchema#string">TA0021</ns1:valueCode>
    <rdfs:subClassOf rdf:resource="https://m82-project.org/dima-bias/ontology#InformTactic"/>
    <rdfs:label xml:lang="en">Pattern creation</rdfs:label>
    <rdfs:label xml:lang="fr">Création d’un motif</rdfs:label>
  </rdf:Description>
  <rdf:Description rdf:about="https://m82-project.org/dima-bias/ontology#InformTechnique">
    <rdfs:label xml:lang="en">Inform technique</rdfs:label>
    <rdfs:comment xml:lang="en">Techniques that belong to Inform‑phase tactics.</rdfs:comment>
    <rdfs:subClassOf rdf:resource="https://m82-project.org/dima-bias/ontology#Technique"/>
    <rdfs:subClassOf rdf:nodeID="N0dfd6d192ebd470799ad4cb1d92a5643"/>
    <rdfs:subClassOf rdf:nodeID="N22c0e651bced47ae8a760c09bf6f9bfc"/>
    <rdf:type rdf:resource="http://www.w3.org/2002/07/owl#Class"/>
  </rdf:Description>
  <rdf:Description rdf:about="https://m82-project.org/dima-bias/ontology#c9ce7d9bb7_negativitybias_4">
    <ns1:instantiatesTechnique rdf:resource="https://m82-project.org/dima-bias/ontology#NegativityBias"/>
    <ns1:hasExplanation rdf:datatype="http://www.w3.org/2001/XMLSchema#string">Both premises frame the situation in negative terms (disruption, tension) without neutral or positive balance, emphasizing threat and instability to exploit negativity bias.</ns1:hasExplanation>
    <rdf:type rdf:resource="http://www.w3.org/2002/07/owl#NamedIndividual"/>
    <rdf:type rdf:resource="https://m82-project.org/dima-bias/ontology#TechniqueUsage"/>
  </rdf:Description>
  <rdf:Description rdf:about="https://m82-project.org/dima-bias/ontology#InformationOverload">
    <rdf:type rdf:resource="https://m82-project.org/dima-bias/ontology#ActTechnique"/>
    <rdf:type rdf:resource="http://www.w3.org/2002/07/owl#Class"/>
    <rdf:type rdf:resource="http://www.w3.org/2002/07/owl#NamedIndividual"/>
    <rdf:type rdf:resource="https://m82-project.org/dima-bias/ontology#Technique"/>
    <rdfs:subClassOf rdf:resource="https://m82-project.org/dima-bias/ontology#ActTechnique"/>
    <rdfs:label xml:lang="fr">Saturation informationnelle</rdfs:label>
    <rdfs:label xml:lang="en">information overload</rdfs:label>
    <rdfs:comment xml:lang="en">Overloading a target with information to disrupt decision-making (analysis paralysis).</rdfs:comment>
    <rdfs:comment xml:lang="fr">Saturation de la cible d’informations afin de paralyser la prise de décision.</rdfs:comment>
    <ns1:valueCode rdf:datatype="http://www.w3.org/2001/XMLSchema#string">TE0433</ns1:valueCode>
  </rdf:Description>
  <rdf:Description rdf:about="https://m82-project.org/dima-bias/ontology#ActArgument">
    <rdfs:label xml:lang="en">Act argument</rdfs:label>
    <owl:equivalentClass rdf:nodeID="N3f1b26f14a544e87be25c61f7c7146fd"/>
    <owl:equivalentClass rdf:nodeID="N41749741d84444f2a8f45fafa256c0fc"/>
    <rdf:type rdf:resource="http://www.w3.org/2002/07/owl#Class"/>
    <rdfs:comment xml:lang="en">Arguments that use techniques from the Act phase.</rdfs:comment>
  </rdf:Description>
  <rdf:Description rdf:about="https://m82-project.org/dima-bias/ontology#ContentExposure">
    <ns1:valueCode rdf:datatype="http://www.w3.org/2001/XMLSchema#string">TA0033</ns1:valueCode>
    <rdf:type rdf:resource="http://www.w3.org/2002/07/owl#Class"/>
    <rdf:type rdf:resource="http://www.w3.org/2002/07/owl#NamedIndividual"/>
    <rdf:type rdf:resource="https://m82-project.org/dima-bias/ontology#MemoriseTactic"/>
    <rdf:type rdf:resource="https://m82-project.org/dima-bias/ontology#Tactic"/>
    <rdfs:label xml:lang="fr">Exposition de contenus</rdfs:label>
    <rdfs:label xml:lang="en">Content exposure</rdfs:label>
    <rdfs:comment xml:lang="en">A tactic that promotes memorization through overexposure to information.</rdfs:comment>
    <rdfs:comment xml:lang="fr">Tactique qui favorise la surexposition à une information pour favoriser sa mémorisation.</rdfs:comment>
    <ns1:hasTechnique rdf:resource="https://m82-project.org/dima-bias/ontology#RecencyEffect"/>
    <ns1:hasTechnique rdf:resource="https://m82-project.org/dima-bias/ontology#MereExposureEffect_Memorise"/>
    <ns1:hasTechnique rdf:resource="https://m82-project.org/dima-bias/ontology#PrimacyEffect"/>
    <rdfs:subClassOf rdf:resource="https://m82-project.org/dima-bias/ontology#MemoriseTactic"/>
  </rdf:Description>
  <rdf:Description rdf:about="https://m82-project.org/dima-bias/ontology#c9ce7d9bb7_vonrestorffeffect_3">
    <rdf:type rdf:resource="https://m82-project.org/dima-bias/ontology#TechniqueUsage"/>
    <rdf:type rdf:resource="http://www.w3.org/2002/07/owl#NamedIndividual"/>
    <ns1:instantiatesTechnique rdf:resource="https://m82-project.org/dima-bias/ontology#VonRestorffEffect"/>
    <ns1:hasExplanation rdf:datatype="http://www.w3.org/2001/XMLSchema#string">The use of direct quotations from a named individual, set apart from the general narrative, isolates these statements and makes them stand out, exploiting the Von Restorff Effect to make the support and defiance more memorable.</ns1:hasExplanation>
  </rdf:Description>
  <rdf:Description rdf:about="https://m82-project.org/dima-bias/ontology#usesTechnique">
    <rdfs:label xml:lang="en">uses technique</rdfs:label>
    <rdfs:label xml:lang="fr">utilise une technique</rdfs:label>
    <rdfs:comment xml:lang="en">Links an argument to a TechniqueUsage node that represents a concrete use of a technique.</rdfs:comment>
    <rdfs:comment xml:lang="fr">Associe un argument à un nœud TechniqueUsage qui représente un usage concret d’une technique.</rdfs:comment>
    <rdfs:domain rdf:resource="https://stratcomcoe.org/influence-mini/ontology#Argument"/>
    <owl:inverseOf rdf:resource="https://m82-project.org/dima-bias/ontology#isTechniqueUsedBy"/>
    <rdfs:range rdf:resource="https://m82-project.org/dima-bias/ontology#TechniqueUsage"/>
    <rdf:type rdf:resource="http://www.w3.org/2002/07/owl#ObjectProperty"/>
  </rdf:Description>
  <rdf:Description rdf:about="https://m82-project.org/dima-bias/ontology#DetectTactic">
    <rdfs:comment xml:lang="en">Tactics associated with the Detect phase.</rdfs:comment>
    <rdfs:subClassOf rdf:resource="https://m82-project.org/dima-bias/ontology#Tactic"/>
    <rdfs:subClassOf rdf:nodeID="N380ad3e10604473f9422c50c47973d2c"/>
    <rdfs:subClassOf rdf:nodeID="Ndfa9e2299c7140b89e8f5576a1b9aa8c"/>
    <rdf:type rdf:resource="http://www.w3.org/2002/07/owl#Class"/>
    <rdfs:label xml:lang="en">Detect tactic</rdfs:label>
  </rdf:Description>
  <rdf:Description rdf:about="https://m82-project.org/dima-bias/ontology#9a2a4d3a26_hindsightbias_2">
    <rdf:type rdf:resource="http://www.w3.org/2002/07/owl#NamedIndividual"/>
    <rdf:type rdf:resource="https://m82-project.org/dima-bias/ontology#TechniqueUsage"/>
    <ns1:hasExplanation rdf:datatype="http://www.w3.org/2001/XMLSchema#string">The argument retroactively claims that warning signs were clear from the start, presenting the outcome as predictable despite acknowledging it was not obvious before.</ns1:hasExplanation>
    <ns1:instantiatesTechnique rdf:resource="https://m82-project.org/dima-bias/ontology#HindsightBias"/>
  </rdf:Description>
  <rdf:Description rdf:about="https://m82-project.org/dima-bias/ontology#hasTechnique">
    <rdfs:domain rdf:resource="https://m82-project.org/dima-bias/ontology#Tactic"/>
    <rdfs:label xml:lang="en">has technique</rdfs:label>
    <rdfs:label xml:lang="fr">possède une technique</rdfs:label>
    <rdf:type rdf:resource="http://www.w3.org/2002/07/owl#ObjectProperty"/>
    <rdfs:comment xml:lang="fr">Relie une tactique narrative à une ou plusieurs techniques cognitives.</rdfs:comment>
    <rdfs:comment xml:lang="en">Links a narrative tactic to one or more cognitive techniques.</rdfs:comment>
    <rdfs:range rdf:resource="https://m82-project.org/dima-bias/ontology#Technique"/>
  </rdf:Description>
  <rdf:Description rdf:about="https://m82-project.org/dima-bias/ontology#TemporalProjection">
    <rdfs:comment xml:lang="en">A tactic that draws on (real or fabricated) memories to legitimize a message.</rdfs:comment>
    <rdfs:comment xml:lang="fr">Tactique qui s’appuie sur les souvenirs (réels ou forgés) pour crédibiliser un discours ou une information.</rdfs:comment>
    <rdf:type rdf:resource="https://m82-project.org/dima-bias/ontology#Tactic"/>
    <rdf:type rdf:resource="https://m82-project.org/dima-bias/ontology#InformTactic"/>
    <rdf:type rdf:resource="http://www.w3.org/2002/07/owl#Class"/>
    <rdf:type rdf:resource="http://www.w3.org/2002/07/owl#NamedIndividual"/>
    <ns1:valueCode rdf:datatype="http://www.w3.org/2001/XMLSchema#string">TA0026</ns1:valueCode>
    <rdfs:label xml:lang="en">Temporal projection</rdfs:label>
    <rdfs:label xml:lang="fr">Projection temporelle</rdfs:label>
    <rdfs:subClassOf rdf:resource="https://m82-project.org/dima-bias/ontology#InformTactic"/>
    <ns1:hasTechnique rdf:resource="https://m82-project.org/dima-bias/ontology#HindsightBias"/>
  </rdf:Description>
  <rdf:Description rdf:about="https://stratcomcoe.org/influence-mini/ontology#c9ce7d9bb7_argument_1">
    <ns1:usesTechnique rdf:resource="https://m82-project.org/dima-bias/ontology#c9ce7d9bb7_negativitybias_1"/>
    <ns1:usesTechnique rdf:resource="https://m82-project.org/dima-bias/ontology#c9ce7d9bb7_vonrestorffeffect_1"/>
  </rdf:Description>
  <rdf:Description rdf:about="https://m82-project.org/dima-bias/ontology#EscalationReinforcement">
    <rdf:type rdf:resource="https://m82-project.org/dima-bias/ontology#ActTactic"/>
    <rdf:type rdf:resource="http://www.w3.org/2002/07/owl#NamedIndividual"/>
    <rdf:type rdf:resource="https://m82-project.org/dima-bias/ontology#Tactic"/>
    <rdf:type rdf:resource="http://www.w3.org/2002/07/owl#Class"/>
    <rdfs:label xml:lang="en">Escalation reinforcement</rdfs:label>
    <rdfs:label xml:lang="fr">Renforcement escalatoire</rdfs:label>
    <rdfs:comment xml:lang="en">A tactic that encourages continuation of actions already initiated.</rdfs:comment>
    <rdfs:comment xml:lang="fr">Tactique qui favorise la réalisation d'actions déjà engagées.</rdfs:comment>
    <ns1:hasTechnique rdf:resource="https://m82-project.org/dima-bias/ontology#AuthorityBias"/>
    <ns1:hasTechnique rdf:resource="https://m82-project.org/dima-bias/ontology#SunkCostBias"/>
    <rdfs:subClassOf rdf:resource="https://m82-project.org/dima-bias/ontology#ActTactic"/>
    <ns1:valueCode rdf:datatype="http://www.w3.org/2001/XMLSchema#string">TA0042</ns1:valueCode>
  </rdf:Description>
  <rdf:Description rdf:nodeID="N520932e1769f4f768078c62acb1eaa8d">
    <owl:someValuesFrom rdf:resource="https://m82-project.org/dima-bias/ontology#Act"/>
    <rdf:type rdf:resource="http://www.w3.org/2002/07/owl#Restriction"/>
    <owl:onProperty rdf:resource="https://m82-project.org/dima-bias/ontology#isTacticOf"/>
  </rdf:Description>
  <rdf:Description rdf:about="https://m82-project.org/dima-bias/ontology#isTacticUsedBy">
    <rdfs:label xml:lang="fr">est utilisée dans un argument (tactique)</rdfs:label>
    <rdfs:label xml:lang="en">is used in argument (tactic)</rdfs:label>
    <rdfs:domain rdf:resource="https://m82-project.org/dima-bias/ontology#Tactic"/>
    <rdfs:comment xml:lang="en">Inverse of inferred property linking a tactic to the arguments that imply it.</rdfs:comment>
    <rdfs:comment xml:lang="fr">Propriété inverse inférée reliant une tactique aux arguments qui l’impliquent.</rdfs:comment>
    <rdfs:range rdf:resource="https://stratcomcoe.org/influence-mini/ontology#Argument"/>
    <rdf:type rdf:resource="http://www.w3.org/2002/07/owl#ObjectProperty"/>
    <owl:inverseOf rdf:resource="https://m82-project.org/dima-bias/ontology#usesTactic"/>
  </rdf:Description>
  <rdf:Description rdf:about="https://m82-project.org/dima-bias/ontology#isTechniqueOf">
    <rdfs:label xml:lang="fr">est une technique de</rdfs:label>
    <rdfs:label xml:lang="en">is technique of</rdfs:label>
    <rdfs:domain rdf:resource="https://m82-project.org/dima-bias/ontology#Technique"/>
    <rdfs:comment xml:lang="fr">Propriété inverse reliant une technique aux tactiques auxquelles elle est associée.</rdfs:comment>
    <rdfs:comment xml:lang="en">Inverse property linking a technique to its associated tactic(s).</rdfs:comment>
    <owl:inverseOf rdf:resource="https://m82-project.org/dima-bias/ontology#hasTechnique"/>
    <rdf:type rdf:resource="http://www.w3.org/2002/07/owl#ObjectProperty"/>
    <rdfs:range rdf:resource="https://m82-project.org/dima-bias/ontology#Tactic"/>
  </rdf:Description>
  <rdf:Description rdf:about="https://m82-project.org/dima-bias/ontology#AnchoringBias">
    <rdf:type rdf:resource="http://www.w3.org/2002/07/owl#NamedIndividual"/>
    <rdf:type rdf:resource="https://m82-project.org/dima-bias/ontology#Technique"/>
    <rdf:type rdf:resource="https://m82-project.org/dima-bias/ontology#DetectTechnique"/>
    <rdf:type rdf:resource="http://www.w3.org/2002/07/owl#Class"/>
    <rdfs:subClassOf rdf:resource="https://m82-project.org/dima-bias/ontology#DetectTechnique"/>
    <rdfs:comment xml:lang="en">Over-reliance on the first piece of information received when making decisions.</rdfs:comment>
    <rdfs:comment xml:lang="fr">Tendance à se fixer sur la première information reçue dans un jugement.</rdfs:comment>
    <rdfs:label xml:lang="en">anchoring bias</rdfs:label>
    <rdfs:label xml:lang="fr">Biais d’ancrage</rdfs:label>
    <ns1:valueCode rdf:datatype="http://www.w3.org/2001/XMLSchema#string">TE0142</ns1:valueCode>
  </rdf:Description>
  <rdf:Description rdf:about="https://m82-project.org/dima-bias/ontology#Simplification">
    <rdfs:comment xml:lang="en">A tactic that simplifies concepts and emphasizes scale to improve information acceptability.</rdfs:comment>
    <rdfs:comment xml:lang="fr">Tactique qui simplifie les concepts et favorise les ordres de grandeurs pour faciliter l'acceptabilité d'une information.</rdfs:comment>
    <rdfs:label xml:lang="fr">Simplification</rdfs:label>
    <rdfs:label xml:lang="en">Simplification</rdfs:label>
    <ns1:hasTechnique rdf:resource="https://m82-project.org/dima-bias/ontology#ZeroSumBias"/>
    <ns1:hasTechnique rdf:resource="https://m82-project.org/dima-bias/ontology#NormalcyBias"/>
    <rdf:type rdf:resource="https://m82-project.org/dima-bias/ontology#InformTactic"/>
    <rdf:type rdf:resource="https://m82-project.org/dima-bias/ontology#Tactic"/>
    <rdf:type rdf:resource="http://www.w3.org/2002/07/owl#Class"/>
    <rdf:type rdf:resource="http://www.w3.org/2002/07/owl#NamedIndividual"/>
    <ns1:valueCode rdf:datatype="http://www.w3.org/2001/XMLSchema#string">TA0024</ns1:valueCode>
    <rdfs:subClassOf rdf:resource="https://m82-project.org/dima-bias/ontology#InformTactic"/>
  </rdf:Description>
  <rdf:Description rdf:about="https://m82-project.org/dima-bias/ontology#MemoriseTechnique">
    <rdfs:subClassOf rdf:resource="https://m82-project.org/dima-bias/ontology#Technique"/>
    <rdfs:subClassOf rdf:nodeID="N1a4d16cb70c347c1b03c11a43f42aa67"/>
    <rdfs:subClassOf rdf:nodeID="Na6028b6e98354559beb5d43db5a02771"/>
    <rdfs:comment xml:lang="en">Techniques that belong to Memorise‑phase tactics.</rdfs:comment>
    <rdf:type rdf:resource="http://www.w3.org/2002/07/owl#Class"/>
    <rdfs:label xml:lang="en">Memorise technique</rdfs:label>
  </rdf:Description>
  <rdf:Description rdf:about="https://m82-project.org/dima-bias/ontology#MereExposureEffect">
    <rdfs:comment xml:lang="fr">Préférence croissante envers ce qui est familier par exposition répétée.</rdfs:comment>
    <rdfs:comment xml:lang="en">Tendency to develop preference for things merely because they are familiar.</rdfs:comment>
    <ns1:valueCode rdf:datatype="http://www.w3.org/2001/XMLSchema#string">TE0112</ns1:valueCode>
    <rdf:type rdf:resource="http://www.w3.org/2002/07/owl#Class"/>
    <rdf:type rdf:resource="http://www.w3.org/2002/07/owl#NamedIndividual"/>
    <rdf:type rdf:resource="https://m82-project.org/dima-bias/ontology#Technique"/>
    <rdf:type rdf:resource="https://m82-project.org/dima-bias/ontology#DetectTechnique"/>
    <rdfs:label xml:lang="fr">Effet de simple exposition</rdfs:label>
    <rdfs:label xml:lang="en">mere exposure effect</rdfs:label>
    <rdfs:subClassOf rdf:resource="https://m82-project.org/dima-bias/ontology#DetectTechnique"/>
  </rdf:Description>
  <rdf:Description rdf:nodeID="N9fb2eddc5e1e4ad5b8664de93ea06ee1">
    <rdf:first rdf:resource="https://m82-project.org/dima-bias/ontology#isTechniqueOf"/>
    <rdf:rest rdf:nodeID="N6091de76c2e54b6491101d5e30e0958d"/>
  </rdf:Description>
  <rdf:Description rdf:nodeID="Nc3e48981dc3d429dbaf9af2e34de2bac">
    <rdf:type rdf:resource="http://www.w3.org/2002/07/owl#Class"/>
    <owl:intersectionOf rdf:nodeID="N2b106c845abe4afbb5b174b0e595a4e3"/>
  </rdf:Description>
  <rdf:Description rdf:about="https://m82-project.org/dima-bias/ontology#isTacticOf">
    <rdfs:comment xml:lang="en">Inverse property linking a tactic to its corresponding DIMA phase.</rdfs:comment>
    <rdfs:comment xml:lang="fr">Propriété inverse associant une tactique à sa phase DIMA correspondante.</rdfs:comment>
    <owl:inverseOf rdf:resource="https://m82-project.org/dima-bias/ontology#hasTactic"/>
    <rdfs:label xml:lang="fr">est une tactique de</rdfs:label>
    <rdfs:label xml:lang="en">is tactic of</rdfs:label>
    <rdf:type rdf:resource="http://www.w3.org/2002/07/owl#ObjectProperty"/>
    <rdfs:domain rdf:resource="https://m82-project.org/dima-bias/ontology#Tactic"/>
    <rdfs:range rdf:resource="https://m82-project.org/dima-bias/ontology#Phase"/>
  </rdf:Description>
  <rdf:Description rdf:about="https://m82-project.org/dima-bias/ontology#WellTraveledRoadBias">
    <rdfs:label xml:lang="fr">Biais de la route connue</rdfs:label>
    <rdfs:label xml:lang="en">well-traveled road bias</rdfs:label>
    <rdf:type rdf:resource="https://m82-project.org/dima-bias/ontology#InformTechnique"/>
    <rdf:type rdf:resource="http://www.w3.org/2002/07/owl#Class"/>
    <rdf:type rdf:resource="http://www.w3.org/2002/07/owl#NamedIndividual"/>
    <rdf:type rdf:resource="https://m82-project.org/dima-bias/ontology#Technique"/>
    <rdfs:comment xml:lang="fr">Préférer ce qui est familier, même si d'autres options sont meilleures.</rdfs:comment>
    <rdfs:comment xml:lang="en">Preferring familiar paths even when others are better.</rdfs:comment>
    <rdfs:subClassOf rdf:resource="https://m82-project.org/dima-bias/ontology#InformTechnique"/>
    <ns1:valueCode rdf:datatype="http://www.w3.org/2001/XMLSchema#string">TE0232</ns1:valueCode>
  </rdf:Description>
  <rdf:Description rdf:about="https://m82-project.org/dima-bias/ontology#isInstantiatedByTechniqueUsage">
    <rdfs:domain rdf:resource="https://m82-project.org/dima-bias/ontology#Technique"/>
    <rdfs:range rdf:resource="https://m82-project.org/dima-bias/ontology#TechniqueUsage"/>
    <rdfs:label xml:lang="fr">a un usage concret</rdfs:label>
    <rdfs:label xml:lang="en">has concrete usage</rdfs:label>
    <rdf:type rdf:resource="http://www.w3.org/2002/07/owl#ObjectProperty"/>
    <rdfs:comment xml:lang="en">Inverse linking a technique to its concrete TechniqueUsage nodes.</rdfs:comment>
    <rdfs:comment xml:lang="fr">Propriété inverse reliant une technique à ses nœuds TechniqueUsage concrets.</rdfs:comment>
  </rdf:Description>
  <rdf:Description rdf:nodeID="N49f63948ff694cd99ff006c0f5cb508a">
    <owl:onProperty rdf:resource="https://m82-project.org/dima-bias/ontology#usesPhase"/>
    <rdf:type rdf:resource="http://www.w3.org/2002/07/owl#Restriction"/>
    <owl:hasValue rdf:resource="https://m82-project.org/dima-bias/ontology#Detect"/>
  </rdf:Description>
  <rdf:Description rdf:about="https://m82-project.org/dima-bias/ontology#PrimacyEffect">
    <rdf:type rdf:resource="https://m82-project.org/dima-bias/ontology#MemoriseTechnique"/>
    <rdf:type rdf:resource="http://www.w3.org/2002/07/owl#Class"/>
    <rdf:type rdf:resource="http://www.w3.org/2002/07/owl#NamedIndividual"/>
    <rdf:type rdf:resource="https://m82-project.org/dima-bias/ontology#Technique"/>
    <rdfs:label xml:lang="en">primacy effect</rdfs:label>
    <rdfs:label xml:lang="fr">Effet de primauté</rdfs:label>
    <rdfs:comment xml:lang="fr">Les premières informations reçues ont un impact durable sur la perception et la mémoire.</rdfs:comment>
    <rdfs:comment xml:lang="en">First information encountered is remembered more easily and influences perception.</rdfs:comment>
    <ns1:valueCode rdf:datatype="http://www.w3.org/2001/XMLSchema#string">TE0333</ns1:valueCode>
    <rdfs:subClassOf rdf:resource="https://m82-project.org/dima-bias/ontology#MemoriseTechnique"/>
  </rdf:Description>
  <rdf:Description rdf:nodeID="N3f1b26f14a544e87be25c61f7c7146fd">
    <owl:intersectionOf rdf:nodeID="N4a19cd0027da40b390e35a83c62e1ccc"/>
    <rdf:type rdf:resource="http://www.w3.org/2002/07/owl#Class"/>
  </rdf:Description>
  <rdf:Description rdf:about="https://m82-project.org/dima-bias/ontology#SunkCostBias">
    <rdfs:label xml:lang="en">sunk cost bias</rdfs:label>
    <rdfs:label xml:lang="fr">biais des coûts irrécupérables</rdfs:label>
    <rdf:type rdf:resource="http://www.w3.org/2002/07/owl#Class"/>
    <rdf:type rdf:resource="http://www.w3.org/2002/07/owl#NamedIndividual"/>
    <rdf:type rdf:resource="https://m82-project.org/dima-bias/ontology#ActTechnique"/>
    <rdf:type rdf:resource="https://m82-project.org/dima-bias/ontology#Technique"/>
    <rdfs:comment xml:lang="fr">Tendance à poursuivre un effort déjà engagé en raison d’un investissement passé.</rdfs:comment>
    <rdfs:comment xml:lang="en">Tendency to continue an endeavor once an investment in money, effort, or time has been made.</rdfs:comment>
    <ns1:valueCode rdf:datatype="http://www.w3.org/2001/XMLSchema#string">TE0421</ns1:valueCode>
    <rdfs:subClassOf rdf:resource="https://m82-project.org/dima-bias/ontology#ActTechnique"/>
  </rdf:Description>
  <rdf:Description rdf:about="https://stratcomcoe.org/influence-mini/ontology#c9ce7d9bb7_conclusion_1">
    <ns1:usesTechnique rdf:resource="https://m82-project.org/dima-bias/ontology#c9ce7d9bb7_vonrestorffeffect_2"/>
    <ns1:usesTechnique rdf:resource="https://m82-project.org/dima-bias/ontology#c9ce7d9bb7_negativitybias_2"/>
  </rdf:Description>
  <rdf:Description rdf:nodeID="N41a4e970c1be445e9c549106a870d510">
    <rdf:first rdf:resource="https://m82-project.org/dima-bias/ontology#isTechniqueOf"/>
    <rdf:rest rdf:resource="http://www.w3.org/1999/02/22-rdf-syntax-ns#nil"/>
  </rdf:Description>
  <rdf:Description rdf:nodeID="N74a246fde62d4e148d6d019bfb27efda">
    <rdf:type rdf:resource="http://www.w3.org/2002/07/owl#Restriction"/>
    <owl:onProperty rdf:resource="https://m82-project.org/dima-bias/ontology#usesPhase"/>
    <owl:hasValue rdf:resource="https://m82-project.org/dima-bias/ontology#Memorise"/>
  </rdf:Description>
  <rdf:Description rdf:nodeID="Nc44f1fe74c6547d1b7a02e1fd09e3b03">
    <owl:someValuesFrom rdf:resource="https://m82-project.org/dima-bias/ontology#Inform"/>
    <rdf:type rdf:resource="http://www.w3.org/2002/07/owl#Restriction"/>
    <owl:onProperty rdf:resource="https://m82-project.org/dima-bias/ontology#isTacticOf"/>
  </rdf:Description>
  <rdf:Description rdf:about="https://m82-project.org/dima-bias/ontology#NormalcyBias">
    <rdfs:subClassOf rdf:resource="https://m82-project.org/dima-bias/ontology#InformTechnique"/>
    <rdfs:label xml:lang="en">normalcy bias</rdfs:label>
    <rdfs:label xml:lang="fr">Biais de normalité</rdfs:label>
    <ns1:valueCode rdf:datatype="http://www.w3.org/2001/XMLSchema#string">TE0242</ns1:valueCode>
    <rdf:type rdf:resource="http://www.w3.org/2002/07/owl#Class"/>
    <rdf:type rdf:resource="http://www.w3.org/2002/07/owl#NamedIndividual"/>
    <rdf:type rdf:resource="https://m82-project.org/dima-bias/ontology#InformTechnique"/>
    <rdf:type rdf:resource="https://m82-project.org/dima-bias/ontology#Technique"/>
    <rdfs:comment xml:lang="fr">Penser que rien ne changera parce que les choses ont toujours été normales.</rdfs:comment>
    <rdfs:comment xml:lang="en">Underestimating the likelihood of a crisis because things have always been normal.</rdfs:comment>
  </rdf:Description>
  <rdf:Description rdf:nodeID="Ndfa9e2299c7140b89e8f5576a1b9aa8c">
    <rdf:type rdf:resource="http://www.w3.org/2002/07/owl#Restriction"/>
    <owl:onProperty rdf:resource="https://m82-project.org/dima-bias/ontology#isTacticOf"/>
    <owl:someValuesFrom rdf:resource="https://m82-project.org/dima-bias/ontology#Detect"/>
  </rdf:Description>
  <rdf:Description rdf:about="https://m82-project.org/dima-bias/ontology#BizarrenessEffect">
    <rdf:type rdf:resource="https://m82-project.org/dima-bias/ontology#DetectTechnique"/>
    <rdf:type rdf:resource="http://www.w3.org/2002/07/owl#Class"/>
    <rdf:type rdf:resource="http://www.w3.org/2002/07/owl#NamedIndividual"/>
    <rdf:type rdf:resource="https://m82-project.org/dima-bias/ontology#Technique"/>
    <rdfs:label xml:lang="fr">Effet de bizarrerie</rdfs:label>
    <rdfs:label xml:lang="en">bizarreness effect</rdfs:label>
    <rdfs:subClassOf rdf:resource="https://m82-project.org/dima-bias/ontology#DetectTechnique"/>
    <ns1:valueCode rdf:datatype="http://www.w3.org/2001/XMLSchema#string">TE0131</ns1:valueCode>
    <rdfs:comment xml:lang="en">Strange or unusual information is more likely to be noticed and remembered.</rdfs:comment>
    <rdfs:comment xml:lang="fr">Tendance à remarquer et mémoriser plus facilement les informations étranges.</rdfs:comment>
  </rdf:Description>
  <rdf:Description rdf:nodeID="Na909bfedb56543d183762981a9d8d78c">
    <rdf:first rdf:resource="https://m82-project.org/dima-bias/ontology#isTechniqueOf"/>
    <rdf:rest rdf:nodeID="Na235b3a192944b1fa04d9a2abff9a4ae"/>
  </rdf:Description>
  <rdf:Description rdf:nodeID="N9b584de0c2d749f5924b8516cc853762">
    <rdf:type rdf:resource="http://www.w3.org/2002/07/owl#Restriction"/>
    <owl:onProperty rdf:resource="https://m82-project.org/dima-bias/ontology#isTacticOf"/>
    <owl:someValuesFrom rdf:resource="https://m82-project.org/dima-bias/ontology#Memorise"/>
  </rdf:Description>
  <rdf:Description rdf:nodeID="N320c12a0b5f04793acfdfb02e53b75c0">
    <rdf:first rdf:resource="https://stratcomcoe.org/influence-mini/ontology#Argument"/>
    <rdf:rest rdf:nodeID="Ne57379dc671f41a2b082e8d1b0c48f18"/>
  </rdf:Description>
  <rdf:Description rdf:about="https://m82-project.org/dima-bias/ontology#Act">
    <rdfs:label xml:lang="en">ACT</rdfs:label>
    <rdfs:label xml:lang="fr">AGIR</rdfs:label>
    <rdfs:subClassOf rdf:resource="https://m82-project.org/dima-bias/ontology#Phase"/>
    <ns1:hasTactic rdf:resource="https://m82-project.org/dima-bias/ontology#OzaekomiWaza"/>
    <ns1:hasTactic rdf:resource="https://m82-project.org/dima-bias/ontology#EscalationReinforcement"/>
    <ns1:hasTactic rdf:resource="https://m82-project.org/dima-bias/ontology#IndividualValorisation"/>
    <rdf:type rdf:resource="http://www.w3.org/2002/07/owl#Class"/>
    <rdf:type rdf:resource="http://www.w3.org/2002/07/owl#NamedIndividual"/>
    <rdf:type rdf:resource="https://m82-project.org/dima-bias/ontology#Phase"/>
  </rdf:Description>
  <rdf:Description rdf:about="https://m82-project.org/dima-bias/ontology#FrequencyIllusion">
    <rdf:type rdf:resource="http://www.w3.org/2002/07/owl#Class"/>
    <rdf:type rdf:resource="http://www.w3.org/2002/07/owl#NamedIndividual"/>
    <rdf:type rdf:resource="https://m82-project.org/dima-bias/ontology#Technique"/>
    <rdf:type rdf:resource="https://m82-project.org/dima-bias/ontology#DetectTechnique"/>
    <rdfs:label xml:lang="fr">Illusion de la fréquence</rdfs:label>
    <rdfs:label xml:lang="en">frequency illusion</rdfs:label>
    <rdfs:comment xml:lang="en">Perception that something occurs more frequently after first noticing it — also called the Baader-Meinhof effect.</rdfs:comment>
    <rdfs:comment xml:lang="fr">Croire qu’un phénomène est plus fréquent après l’avoir remarqué une fois (effet Baader-Meinhof).</rdfs:comment>
    <rdfs:subClassOf rdf:resource="https://m82-project.org/dima-bias/ontology#DetectTechnique"/>
    <ns1:valueCode rdf:datatype="http://www.w3.org/2001/XMLSchema#string">TE0121</ns1:valueCode>
  </rdf:Description>
  <rdf:Description rdf:about="https://stratcomcoe.org/influence-mini/ontology#9a2a4d3a26_development_0">
    <ns1:usesTechnique rdf:resource="https://m82-project.org/dima-bias/ontology#9a2a4d3a26_vonrestorffeffect_0"/>
  </rdf:Description>
  <rdf:Description rdf:nodeID="N80520c26f6fe46da89533b0b41a7fdda">
    <owl:someValuesFrom rdf:resource="https://m82-project.org/dima-bias/ontology#ActTactic"/>
    <rdf:type rdf:resource="http://www.w3.org/2002/07/owl#Restriction"/>
    <owl:onProperty rdf:resource="https://m82-project.org/dima-bias/ontology#isTechniqueOf"/>
  </rdf:Description>
  <rdf:Description rdf:about="https://m82-project.org/dima-bias/ontology#9a2a4d3a26_negativitybias_1">
    <rdf:type rdf:resource="https://m82-project.org/dima-bias/ontology#TechniqueUsage"/>
    <rdf:type rdf:resource="http://www.w3.org/2002/07/owl#NamedIndividual"/>
    <ns1:instantiatesTechnique rdf:resource="https://m82-project.org/dima-bias/ontology#NegativityBias"/>
    <ns1:hasExplanation rdf:datatype="http://www.w3.org/2001/XMLSchema#string">The argument repeatedly frames Zarnia's actions as threatening and destabilizing, emphasizing negative interpretations without neutral or positive balance.</ns1:hasExplanation>
  </rdf:Description>
  <rdf:Description rdf:about="https://stratcomcoe.org/influence-mini/ontology#9a2a4d3a26_premise_3">
    <ns1:usesTechnique rdf:resource="https://m82-project.org/dima-bias/ontology#9a2a4d3a26_vonrestorffeffect_1"/>
    <ns1:usesTechnique rdf:resource="https://m82-project.org/dima-bias/ontology#9a2a4d3a26_negativitybias_1"/>
  </rdf:Description>
  <rdf:Description rdf:about="https://m82-project.org/dima-bias/ontology#MereExposureEffect_Memorise">
    <rdf:type rdf:resource="http://www.w3.org/2002/07/owl#Class"/>
    <rdf:type rdf:resource="http://www.w3.org/2002/07/owl#NamedIndividual"/>
    <rdf:type rdf:resource="https://m82-project.org/dima-bias/ontology#Technique"/>
    <rdf:type rdf:resource="https://m82-project.org/dima-bias/ontology#MemoriseTechnique"/>
    <ns1:valueCode rdf:datatype="http://www.w3.org/2001/XMLSchema#string">TE0332</ns1:valueCode>
    <rdfs:label xml:lang="fr">Effet de simple exposition</rdfs:label>
    <rdfs:label xml:lang="en">mere exposure effect</rdfs:label>
    <rdfs:subClassOf rdf:resource="https://m82-project.org/dima-bias/ontology#MemoriseTechnique"/>
    <rdfs:comment xml:lang="fr">La répétition d'exposition à une information renforce sa mémorisation et son acceptabilité.</rdfs:comment>
    <rdfs:comment xml:lang="en">Repeated exposure to a stimulus increases familiarity and preference.</rdfs:comment>
  </rdf:Description>
  <rdf:Description rdf:nodeID="N6eda40f91b674b0681acd877762669a5">
    <owl:onProperty rdf:resource="https://m82-project.org/dima-bias/ontology#usesPhase"/>
    <owl:hasValue rdf:resource="https://m82-project.org/dima-bias/ontology#Act"/>
    <rdf:type rdf:resource="http://www.w3.org/2002/07/owl#Restriction"/>
  </rdf:Description>
  <rdf:Description rdf:about="https://m82-project.org/dima-bias/ontology#c9ce7d9bb7_vonrestorffeffect_5">
    <ns1:hasExplanation rdf:datatype="http://www.w3.org/2001/XMLSchema#string">The argument isolates Caldria's approach by repeatedly highlighting its emphasis on dialogue and unwavering principles, making these features stand out in contrast to the unfolding situation and thus more memorable.</ns1:hasExplanation>
    <rdf:type rdf:resource="http://www.w3.org/2002/07/owl#NamedIndividual"/>
    <rdf:type rdf:resource="https://m82-project.org/dima-bias/ontology#TechniqueUsage"/>
    <ns1:instantiatesTechnique rdf:resource="https://m82-project.org/dima-bias/ontology#VonRestorffEffect"/>
  </rdf:Description>
  <rdf:Description rdf:about="https://stratcomcoe.org/influence-mini/ontology#c9ce7d9bb7_development_4">
    <ns1:usesTechnique rdf:resource="https://m82-project.org/dima-bias/ontology#c9ce7d9bb7_vonrestorffeffect_2"/>
  </rdf:Description>
  <rdf:Description rdf:nodeID="Na6028b6e98354559beb5d43db5a02771">
    <owl:onProperty rdf:resource="https://m82-project.org/dima-bias/ontology#isTechniqueOf"/>
    <rdf:type rdf:resource="http://www.w3.org/2002/07/owl#Restriction"/>
    <owl:someValuesFrom rdf:resource="https://m82-project.org/dima-bias/ontology#MemoriseTactic"/>
  </rdf:Description>
  <rdf:Description rdf:about="https://m82-project.org/dima-bias/ontology#c9ce7d9bb7_vonrestorffeffect_2">
    <ns1:hasExplanation rdf:datatype="http://www.w3.org/2001/XMLSchema#string">The argument isolates Caldria's restraint by contrasting it with its right to defend itself and by labeling its behavior as a 'textbook case,' making these elements stand out and more memorable through conceptual distinction.</ns1:hasExplanation>
    <rdf:type rdf:resource="http://www.w3.org/2002/07/owl#NamedIndividual"/>
    <rdf:type rdf:resource="https://m82-project.org/dima-bias/ontology#TechniqueUsage"/>
    <ns1:instantiatesTechnique rdf:resource="https://m82-project.org/dima-bias/ontology#VonRestorffEffect"/>
  </rdf:Description>
  <rdf:Description rdf:about="https://m82-project.org/dima-bias/ontology#TechniqueUsage">
    <rdfs:comment xml:lang="en">A concrete occurrence of a technique inside an argument.</rdfs:comment>
    <rdf:type rdf:resource="http://www.w3.org/2002/07/owl#Class"/>
    <rdfs:label xml:lang="en">Technique Usage</rdfs:label>
  </rdf:Description>
  <rdf:Description rdf:about="https://m82-project.org/dima-bias/ontology#MemoriseTactic">
    <rdfs:comment xml:lang="en">Tactics associated with the Memorise phase.</rdfs:comment>
    <rdf:type rdf:resource="http://www.w3.org/2002/07/owl#Class"/>
    <rdfs:label xml:lang="en">Memorise tactic</rdfs:label>
    <rdfs:subClassOf rdf:resource="https://m82-project.org/dima-bias/ontology#Tactic"/>
    <rdfs:subClassOf rdf:nodeID="N9b584de0c2d749f5924b8516cc853762"/>
    <rdfs:subClassOf rdf:nodeID="N4b29a1960af94f3088fb3d147792ddf3"/>
  </rdf:Description>
  <rdf:Description rdf:about="https://stratcomcoe.org/influence-mini/ontology#c9ce7d9bb7_argument_3">
    <ns1:usesTechnique rdf:resource="https://m82-project.org/dima-bias/ontology#c9ce7d9bb7_vonrestorffeffect_3"/>
  </rdf:Description>
  <rdf:Description rdf:about="https://stratcomcoe.org/influence-mini/ontology#c9ce7d9bb7_premise_8">
    <ns1:usesTechnique rdf:resource="https://m82-project.org/dima-bias/ontology#c9ce7d9bb7_negativitybias_4"/>
  </rdf:Description>
  <rdf:Description rdf:nodeID="Ne4e356813f2144a68e4c738cefba274c">
    <owl:someValuesFrom rdf:resource="https://m82-project.org/dima-bias/ontology#Inform"/>
    <rdf:type rdf:resource="http://www.w3.org/2002/07/owl#Restriction"/>
    <owl:onProperty rdf:resource="https://m82-project.org/dima-bias/ontology#isTacticOf"/>
  </rdf:Description>
  <rdf:Description rdf:about="https://m82-project.org/dima-bias/ontology#isTechniqueUsedBy">
    <rdfs:comment xml:lang="en">Inverse property linking a TechniqueUsage node to the argument that contains it.</rdfs:comment>
    <rdfs:comment xml:lang="fr">Propriété inverse reliant un nœud TechniqueUsage à l’argument qui le contient.</rdfs:comment>
    <rdfs:label xml:lang="en">is used in argument</rdfs:label>
    <rdfs:label xml:lang="fr">est utilisée dans un argument</rdfs:label>
    <rdfs:domain rdf:resource="https://m82-project.org/dima-bias/ontology#TechniqueUsage"/>
    <rdfs:range rdf:resource="https://stratcomcoe.org/influence-mini/ontology#Argument"/>
    <rdf:type rdf:resource="http://www.w3.org/2002/07/owl#ObjectProperty"/>
  </rdf:Description>
  <rdf:Description rdf:nodeID="Na7a31e877ba84c8d9acfd3f1ef582379">
    <rdf:type rdf:resource="http://www.w3.org/2002/07/owl#ObjectProperty"/>
    <owl:equivalentProperty rdf:resource="https://m82-project.org/dima-bias/ontology#usesTactic"/>
    <owl:propertyChainAxiom rdf:nodeID="Nf6e4215a84c74a778294f9d4afad24a8"/>
  </rdf:Description>
  <rdf:Description rdf:nodeID="N733501697ecc44f49b02629043b0e5d1">
    <rdf:first rdf:resource="https://m82-project.org/dima-bias/ontology#instantiatesTechnique"/>
    <rdf:rest rdf:nodeID="N41a4e970c1be445e9c549106a870d510"/>
  </rdf:Description>
  <rdf:Description rdf:nodeID="N944ff1df99794d228a1fce9758f78edf">
    <owl:intersectionOf rdf:nodeID="N7a08789e02de49b88ddb902e512e60f6"/>
    <rdf:type rdf:resource="http://www.w3.org/2002/07/owl#Class"/>
  </rdf:Description>
  <rdf:Description rdf:about="https://m82-project.org/dima-bias/ontology#usesPhase">
    <rdfs:label xml:lang="en">uses phase</rdfs:label>
    <rdfs:label xml:lang="fr">utilise une phase</rdfs:label>
    <rdfs:comment xml:lang="en">Inferred property: links an argument to a DIMA phase via technique and tactic.</rdfs:comment>
    <rdfs:comment xml:lang="fr">Propriété inférée : associe un argument à une phase DIMA via la technique et la tactique.</rdfs:comment>
    <rdfs:domain rdf:resource="https://stratcomcoe.org/influence-mini/ontology#Argument"/>
    <rdf:type rdf:resource="http://www.w3.org/2002/07/owl#ObjectProperty"/>
    <rdfs:range rdf:resource="https://m82-project.org/dima-bias/ontology#Phase"/>
  </rdf:Description>
  <rdf:Description rdf:nodeID="Nd3fafb67c04f43dea9a78f012967ae24">
    <owl:onProperty rdf:resource="https://m82-project.org/dima-bias/ontology#isTechniqueOf"/>
    <rdf:type rdf:resource="http://www.w3.org/2002/07/owl#Restriction"/>
    <owl:someValuesFrom rdf:resource="https://m82-project.org/dima-bias/ontology#DetectTactic"/>
  </rdf:Description>
  <rdf:Description rdf:nodeID="Ne57379dc671f41a2b082e8d1b0c48f18">
    <rdf:first rdf:nodeID="Nb133f359893d4ef3a9a24ec98c601c99"/>
    <rdf:rest rdf:resource="http://www.w3.org/1999/02/22-rdf-syntax-ns#nil"/>
  </rdf:Description>
  <rdf:Description rdf:nodeID="Nf6622a7a9046414dbe83069585aecb6d">
    <rdf:first rdf:nodeID="Ne40830e8d0b640279e9d2d7577ab07bf"/>
    <rdf:rest rdf:resource="http://www.w3.org/1999/02/22-rdf-syntax-ns#nil"/>
  </rdf:Description>
  <rdf:Description rdf:nodeID="N22c0e651bced47ae8a760c09bf6f9bfc">
    <owl:someValuesFrom rdf:resource="https://m82-project.org/dima-bias/ontology#InformTactic"/>
    <owl:onProperty rdf:resource="https://m82-project.org/dima-bias/ontology#isTechniqueOf"/>
    <rdf:type rdf:resource="http://www.w3.org/2002/07/owl#Restriction"/>
  </rdf:Description>
  <rdf:Description rdf:nodeID="N89ff6e16b09b492a82374fce32449caa">
    <rdf:rest rdf:nodeID="Nbbbfe1fd0a7141f1b544222281476f4d"/>
    <rdf:first rdf:resource="https://stratcomcoe.org/influence-mini/ontology#Argument"/>
  </rdf:Description>
  <rdf:Description rdf:about="https://m82-project.org/dima-bias/ontology#VonRestorffEffect">
    <rdfs:comment xml:lang="en">Unusual or distinctive items are more likely to be remembered (isolation effect).</rdfs:comment>
    <rdfs:comment xml:lang="fr">Ce qui se distingue du reste est mieux retenu en mémoire (effet d’isolement).</rdfs:comment>
    <rdf:type rdf:resource="http://www.w3.org/2002/07/owl#Class"/>
    <rdf:type rdf:resource="https://m82-project.org/dima-bias/ontology#DetectTechnique"/>
    <rdf:type rdf:resource="http://www.w3.org/2002/07/owl#NamedIndividual"/>
    <rdf:type rdf:resource="https://m82-project.org/dima-bias/ontology#Technique"/>
    <rdfs:subClassOf rdf:resource="https://m82-project.org/dima-bias/ontology#DetectTechnique"/>
    <ns1:valueCode rdf:datatype="http://www.w3.org/2001/XMLSchema#string">TE0141</ns1:valueCode>
    <rdfs:label xml:lang="fr">Effet von Restorff</rdfs:label>
    <rdfs:label xml:lang="en">von Restorff effect</rdfs:label>
  </rdf:Description>
  <rdf:Description rdf:nodeID="Ndb0a7ab8e9f14a40bf633c3405800dde">
    <rdf:type rdf:resource="http://www.w3.org/2002/07/owl#ObjectProperty"/>
    <owl:equivalentProperty rdf:resource="https://m82-project.org/dima-bias/ontology#usesPhase"/>
    <owl:propertyChainAxiom rdf:nodeID="Nddf0f9609d74475eb32ebda5a0421dbd"/>
  </rdf:Description>
  <rdf:Description rdf:about="https://stratcomcoe.org/influence-mini/ontology#c9ce7d9bb7_development_1">
    <ns1:usesTechnique rdf:resource="https://m82-project.org/dima-bias/ontology#c9ce7d9bb7_vonrestorffeffect_0"/>
  </rdf:Description>
  <rdf:Description rdf:about="https://m82-project.org/dima-bias/ontology#9a2a4d3a26_vonrestorffeffect_0">
    <ns1:instantiatesTechnique rdf:resource="https://m82-project.org/dima-bias/ontology#VonRestorffEffect"/>
    <rdf:type rdf:resource="http://www.w3.org/2002/07/owl#NamedIndividual"/>
    <rdf:type rdf:resource="https://m82-project.org/dima-bias/ontology#TechniqueUsage"/>
    <ns1:hasExplanation rdf:datatype="http://www.w3.org/2001/XMLSchema#string">The argument repeatedly isolates Norlund's peacefulness and restraint as distinct and memorable qualities, contrasting them with Zarnia's provocations to make Norlund's actions stand out.</ns1:hasExplanation>
  </rdf:Description>
  <rdf:Description rdf:about="https://m82-project.org/dima-bias/ontology#FamiliaritySuperiority">
    <rdf:type rdf:resource="http://www.w3.org/2002/07/owl#Class"/>
    <rdf:type rdf:resource="http://www.w3.org/2002/07/owl#NamedIndividual"/>
    <rdf:type rdf:resource="https://m82-project.org/dima-bias/ontology#InformTactic"/>
    <rdf:type rdf:resource="https://m82-project.org/dima-bias/ontology#Tactic"/>
    <rdfs:label xml:lang="en">Familiarity superiority</rdfs:label>
    <rdfs:label xml:lang="fr">Supériorité familière</rdfs:label>
    <rdfs:comment xml:lang="fr">Tactique qui permet de valoriser une information aux yeux de la cible par exploitation des proximités.</rdfs:comment>
    <rdfs:comment xml:lang="en">A tactic that enhances the perceived value of information through familiarity or proximity.</rdfs:comment>
    <rdfs:subClassOf rdf:resource="https://m82-project.org/dima-bias/ontology#InformTactic"/>
    <ns1:hasTechnique rdf:resource="https://m82-project.org/dima-bias/ontology#WellTraveledRoadBias"/>
    <ns1:hasTechnique rdf:resource="https://m82-project.org/dima-bias/ontology#HomogeneityBias"/>
    <ns1:valueCode rdf:datatype="http://www.w3.org/2001/XMLSchema#string">TA0023</ns1:valueCode>
  </rdf:Description>
  <rdf:Description rdf:nodeID="N0dfd6d192ebd470799ad4cb1d92a5643">
    <owl:someValuesFrom rdf:resource="https://m82-project.org/dima-bias/ontology#InformTactic"/>
    <owl:onProperty rdf:resource="https://m82-project.org/dima-bias/ontology#isTechniqueOf"/>
    <rdf:type rdf:resource="http://www.w3.org/2002/07/owl#Restriction"/>
  </rdf:Description>
  <rdf:Description rdf:about="https://stratcomcoe.org/influence-mini/ontology#9a2a4d3a26_premise_9">
    <ns1:usesTechnique rdf:resource="https://m82-project.org/dima-bias/ontology#9a2a4d3a26_negativitybias_3"/>
  </rdf:Description>
  <rdf:Description rdf:nodeID="N6091de76c2e54b6491101d5e30e0958d">
    <rdf:rest rdf:resource="http://www.w3.org/1999/02/22-rdf-syntax-ns#nil"/>
    <rdf:first rdf:resource="https://m82-project.org/dima-bias/ontology#isTacticOf"/>
  </rdf:Description>
  <rdf:Description rdf:about="https://stratcomcoe.org/influence-mini/ontology#c9ce7d9bb7_conclusion_3">
    <ns1:usesTechnique rdf:resource="https://m82-project.org/dima-bias/ontology#c9ce7d9bb7_vonrestorffeffect_5"/>
  </rdf:Description>
  <rdf:Description rdf:nodeID="Nddf0f9609d74475eb32ebda5a0421dbd">
    <rdf:rest rdf:nodeID="N94876565c798488ca0503826143a59f5"/>
    <rdf:first rdf:resource="https://m82-project.org/dima-bias/ontology#usesTechnique"/>
  </rdf:Description>
  <rdf:Description rdf:nodeID="Nab439232d0534c39bf9854ea913073f6">
    <rdf:rest rdf:resource="http://www.w3.org/1999/02/22-rdf-syntax-ns#nil"/>
    <rdf:first rdf:nodeID="N74a246fde62d4e148d6d019bfb27efda"/>
  </rdf:Description>
  <rdf:Description rdf:about="https://stratcomcoe.org/influence-mini/ontology#9a2a4d3a26_premise_7">
    <ns1:usesTechnique rdf:resource="https://m82-project.org/dima-bias/ontology#9a2a4d3a26_hindsightbias_2"/>
    <ns1:usesTechnique rdf:resource="https://m82-project.org/dima-bias/ontology#9a2a4d3a26_vonrestorffeffect_2"/>
  </rdf:Description>
  <rdf:Description rdf:about="https://m82-project.org/dima-bias/ontology#c9ce7d9bb7_negativitybias_1">
    <ns1:instantiatesTechnique rdf:resource="https://m82-project.org/dima-bias/ontology#NegativityBias"/>
    <rdf:type rdf:resource="http://www.w3.org/2002/07/owl#NamedIndividual"/>
    <rdf:type rdf:resource="https://m82-project.org/dima-bias/ontology#TechniqueUsage"/>
    <ns1:hasExplanation rdf:datatype="http://www.w3.org/2001/XMLSchema#string">The argument repeatedly frames Velmora's actions as threats and provocations, emphasizing negative consequences and expert warnings without neutral or positive balance.</ns1:hasExplanation>
  </rdf:Description>
  <rdf:Description rdf:nodeID="N878513753ee046b2947ec74c99988d1e">
    <rdf:first rdf:resource="https://m82-project.org/dima-bias/ontology#usesTechnique"/>
    <rdf:rest rdf:nodeID="N733501697ecc44f49b02629043b0e5d1"/>
  </rdf:Description>
  <rdf:Description rdf:about="https://m82-project.org/dima-bias/ontology#9a2a4d3a26_vonrestorffeffect_2">
    <rdf:type rdf:resource="http://www.w3.org/2002/07/owl#NamedIndividual"/>
    <rdf:type rdf:resource="https://m82-project.org/dima-bias/ontology#TechniqueUsage"/>
    <ns1:hasExplanation rdf:datatype="http://www.w3.org/2001/XMLSchema#string">The direct quote from a named local resident is isolated within the argument, making it stand out and be more memorable compared to the general statement, thus exploiting the Von Restorff Effect.</ns1:hasExplanation>
    <ns1:instantiatesTechnique rdf:resource="https://m82-project.org/dima-bias/ontology#VonRestorffEffect"/>
  </rdf:Description>
  <rdf:Description rdf:about="https://m82-project.org/dima-bias/ontology#uuid">
    <rdfs:comment xml:lang="fr">Identifiant unique et stable issu de la taxonomie source.</rdfs:comment>
    <rdfs:comment xml:lang="en">Stable unique identifier from the original taxonomy source.</rdfs:comment>
    <rdfs:label xml:lang="en">UUID</rdfs:label>
    <rdfs:label xml:lang="fr">UUID</rdfs:label>
    <rdf:type rdf:resource="http://www.w3.org/2002/07/owl#AnnotationProperty"/>
  </rdf:Description>
  <rdf:Description rdf:nodeID="Nb56a79dc40d44d74a85bcfd51d0c51f0">
    <rdf:first rdf:nodeID="N5e3f3ec777cf49208d0c8ed8d42495dd"/>
    <rdf:rest rdf:resource="http://www.w3.org/1999/02/22-rdf-syntax-ns#nil"/>
  </rdf:Description>
  <rdf:Description rdf:about="https://stratcomcoe.org/influence-mini/ontology#c9ce7d9bb7_argument_2">
    <ns1:usesTechnique rdf:resource="https://m82-project.org/dima-bias/ontology#c9ce7d9bb7_vonrestorffeffect_2"/>
    <ns1:usesTechnique rdf:resource="https://m82-project.org/dima-bias/ontology#c9ce7d9bb7_negativitybias_2"/>
  </rdf:Description>
  <rdf:Description rdf:nodeID="Nc40fc7b387344e6a9246b76b6db2ba2f">
    <rdf:type rdf:resource="http://www.w3.org/2002/07/owl#ObjectProperty"/>
    <owl:equivalentProperty rdf:resource="https://m82-project.org/dima-bias/ontology#usesPhase"/>
    <owl:propertyChainAxiom rdf:nodeID="N10a1167eb3a34bd384b68503c6412474"/>
  </rdf:Description>
  <rdf:Description rdf:nodeID="Nd50a1a8a4dbd4010a14d2c09d3d5538d">
    <rdf:rest rdf:resource="http://www.w3.org/1999/02/22-rdf-syntax-ns#nil"/>
    <rdf:first rdf:nodeID="Nca1fd162941d4763a4745646f49a2841"/>
  </rdf:Description>
  <rdf:Description rdf:nodeID="Nf6e4215a84c74a778294f9d4afad24a8">
    <rdf:first rdf:resource="https://m82-project.org/dima-bias/ontology#usesTechnique"/>
    <rdf:rest rdf:nodeID="Nca28e5b4a7bc4d38b8ebf9364eaf1a4d"/>
  </rdf:Description>
  <rdf:Description rdf:nodeID="Nca28e5b4a7bc4d38b8ebf9364eaf1a4d">
    <rdf:first rdf:resource="https://m82-project.org/dima-bias/ontology#instantiatesTechnique"/>
    <rdf:rest rdf:nodeID="Ncf7c353bb1a542b2a7d0cffc91b34b12"/>
  </rdf:Description>
  <rdf:Description rdf:about="https://stratcomcoe.org/influence-mini/ontology#9a2a4d3a26_argument_1">
    <ns1:usesTechnique rdf:resource="https://m82-project.org/dima-bias/ontology#9a2a4d3a26_negativitybias_1"/>
    <ns1:usesTechnique rdf:resource="https://m82-project.org/dima-bias/ontology#9a2a4d3a26_vonrestorffeffect_1"/>
  </rdf:Description>
  <rdf:Description rdf:nodeID="N153767bfc4ce4886a7dbc593be53478d">
    <owl:someValuesFrom rdf:resource="https://m82-project.org/dima-bias/ontology#DetectTactic"/>
    <owl:onProperty rdf:resource="https://m82-project.org/dima-bias/ontology#isTechniqueOf"/>
    <rdf:type rdf:resource="http://www.w3.org/2002/07/owl#Restriction"/>
  </rdf:Description>
  <rdf:Description rdf:about="https://m82-project.org/dima-bias/ontology#hasExplanation">
    <rdfs:label xml:lang="en">has explanation</rdfs:label>
    <rdfs:range rdf:resource="http://www.w3.org/2001/XMLSchema#string"/>
    <rdfs:domain rdf:resource="https://m82-project.org/dima-bias/ontology#TechniqueUsage"/>
    <rdf:type rdf:resource="http://www.w3.org/2002/07/owl#DatatypeProperty"/>
    <rdfs:comment xml:lang="en">Natural‑language explanation attached to a TechniqueUsage node.</rdfs:comment>
  </rdf:Description>
  <rdf:Description rdf:nodeID="N4b29a1960af94f3088fb3d147792ddf3">
    <owl:someValuesFrom rdf:resource="https://m82-project.org/dima-bias/ontology#Memorise"/>
    <rdf:type rdf:resource="http://www.w3.org/2002/07/owl#Restriction"/>
    <owl:onProperty rdf:resource="https://m82-project.org/dima-bias/ontology#isTacticOf"/>
  </rdf:Description>
  <rdf:Description rdf:about="https://stratcomcoe.org/influence-mini/ontology#9a2a4d3a26_conclusion_3">
    <ns1:usesTechnique rdf:resource="https://m82-project.org/dima-bias/ontology#9a2a4d3a26_negativitybias_3"/>
  </rdf:Description>
  <rdf:Description rdf:about="https://m82-project.org/dima-bias/ontology#instantiatesTechnique">
    <rdfs:label xml:lang="en">instantiates technique</rdfs:label>
    <rdfs:label xml:lang="fr">instancie la technique</rdfs:label>
    <rdfs:domain rdf:resource="https://m82-project.org/dima-bias/ontology#TechniqueUsage"/>
    <owl:inverseOf rdf:resource="https://m82-project.org/dima-bias/ontology#isInstantiatedByTechniqueUsage"/>
    <rdfs:range rdf:resource="https://m82-project.org/dima-bias/ontology#Technique"/>
    <rdfs:comment xml:lang="fr">Relie un nœud TechniqueUsage à la technique cognitive qu’il instancie.</rdfs:comment>
    <rdfs:comment xml:lang="en">Connects a TechniqueUsage node to the abstract cognitive technique it instantiates.</rdfs:comment>
    <rdf:type rdf:resource="http://www.w3.org/2002/07/owl#ObjectProperty"/>
  </rdf:Description>
  <rdf:Description rdf:nodeID="Nc77ef51d70854f7d8d046e98ada7b840">
    <rdf:rest rdf:resource="http://www.w3.org/1999/02/22-rdf-syntax-ns#nil"/>
    <rdf:first rdf:nodeID="N49f63948ff694cd99ff006c0f5cb508a"/>
  </rdf:Description>
  <rdf:Description rdf:nodeID="N7a08789e02de49b88ddb902e512e60f6">
    <rdf:first rdf:resource="https://stratcomcoe.org/influence-mini/ontology#Argument"/>
    <rdf:rest rdf:nodeID="Nc77ef51d70854f7d8d046e98ada7b840"/>
  </rdf:Description>
  <rdf:Description rdf:nodeID="N182955c727594ac287dfefec74b37386">
    <rdf:rest rdf:nodeID="N9fb2eddc5e1e4ad5b8664de93ea06ee1"/>
    <rdf:first rdf:resource="https://m82-project.org/dima-bias/ontology#instantiatesTechnique"/>
  </rdf:Description>
  <rdf:Description rdf:nodeID="Na4b452aee43c4317a1a113980770d9e4">
    <owl:someValuesFrom rdf:resource="https://m82-project.org/dima-bias/ontology#Act"/>
    <rdf:type rdf:resource="http://www.w3.org/2002/07/owl#Restriction"/>
    <owl:onProperty rdf:resource="https://m82-project.org/dima-bias/ontology#isTacticOf"/>
  </rdf:Description>
  <rdf:Description rdf:about="https://stratcomcoe.org/influence-mini/ontology#9a2a4d3a26_premise_0">
    <ns1:usesTechnique rdf:resource="https://m82-project.org/dima-bias/ontology#9a2a4d3a26_vonrestorffeffect_0"/>
  </rdf:Description>
  <rdf:Description rdf:about="https://stratcomcoe.org/influence-mini/ontology#9a2a4d3a26_conclusion_2">
    <ns1:usesTechnique rdf:resource="https://m82-project.org/dima-bias/ontology#9a2a4d3a26_hindsightbias_2"/>
  </rdf:Description>
  <rdf:Description rdf:nodeID="Na235b3a192944b1fa04d9a2abff9a4ae">
    <rdf:rest rdf:resource="http://www.w3.org/1999/02/22-rdf-syntax-ns#nil"/>
    <rdf:first rdf:resource="https://m82-project.org/dima-bias/ontology#isTacticOf"/>
  </rdf:Description>
  <rdf:Description rdf:nodeID="N2b106c845abe4afbb5b174b0e595a4e3">
    <rdf:first rdf:resource="https://stratcomcoe.org/influence-mini/ontology#Argument"/>
    <rdf:rest rdf:nodeID="Nb56a79dc40d44d74a85bcfd51d0c51f0"/>
  </rdf:Description>
  <rdf:Description rdf:about="https://stratcomcoe.org/influence-mini/ontology#9a2a4d3a26_argument_0">
    <ns1:usesTechnique rdf:resource="https://m82-project.org/dima-bias/ontology#9a2a4d3a26_vonrestorffeffect_0"/>
  </rdf:Description>
  <rdf:Description rdf:nodeID="N45cb9850dc764c98a0ca5a128d803dc9">
    <rdf:type rdf:resource="http://www.w3.org/2002/07/owl#Restriction"/>
    <owl:someValuesFrom rdf:resource="https://m82-project.org/dima-bias/ontology#ActTactic"/>
    <owl:onProperty rdf:resource="https://m82-project.org/dima-bias/ontology#isTechniqueOf"/>
  </rdf:Description>
  <rdf:Description rdf:nodeID="N1a4d16cb70c347c1b03c11a43f42aa67">
    <owl:someValuesFrom rdf:resource="https://m82-project.org/dima-bias/ontology#MemoriseTactic"/>
    <owl:onProperty rdf:resource="https://m82-project.org/dima-bias/ontology#isTechniqueOf"/>
    <rdf:type rdf:resource="http://www.w3.org/2002/07/owl#Restriction"/>
  </rdf:Description>
  <rdf:Description rdf:nodeID="N7ea66da8323b4064bf01904e8fa8cd0b">
    <owl:equivalentProperty rdf:resource="https://m82-project.org/dima-bias/ontology#usesTactic"/>
    <rdf:type rdf:resource="http://www.w3.org/2002/07/owl#ObjectProperty"/>
    <owl:propertyChainAxiom rdf:nodeID="N878513753ee046b2947ec74c99988d1e"/>
  </rdf:Description>
  <rdf:Description rdf:about="https://stratcomcoe.org/influence-mini/ontology#c9ce7d9bb7_development_5">
    <ns1:usesTechnique rdf:resource="https://m82-project.org/dima-bias/ontology#c9ce7d9bb7_vonrestorffeffect_3"/>
  </rdf:Description>
  <rdf:Description rdf:nodeID="Na136a50d2c1842e3bb5aef3422227dfe">
    <rdf:first rdf:resource="https://stratcomcoe.org/influence-mini/ontology#Argument"/>
    <rdf:rest rdf:nodeID="Nab439232d0534c39bf9854ea913073f6"/>
  </rdf:Description>
  <rdf:Description rdf:nodeID="Ne40830e8d0b640279e9d2d7577ab07bf">
    <rdf:type rdf:resource="http://www.w3.org/2002/07/owl#Restriction"/>
    <owl:onProperty rdf:resource="https://m82-project.org/dima-bias/ontology#usesPhase"/>
    <owl:hasValue rdf:resource="https://m82-project.org/dima-bias/ontology#Memorise"/>
  </rdf:Description>
  <rdf:Description rdf:about="https://stratcomcoe.org/influence-mini/ontology#c9ce7d9bb7_argument_4">
    <ns1:usesTechnique rdf:resource="https://m82-project.org/dima-bias/ontology#c9ce7d9bb7_negativitybias_4"/>
    <ns1:usesTechnique rdf:resource="https://m82-project.org/dima-bias/ontology#c9ce7d9bb7_vonrestorffeffect_4"/>
  </rdf:Description>
  <rdf:Description rdf:about="https://stratcomcoe.org/influence-mini/ontology#c9ce7d9bb7_premise_6">
    <ns1:usesTechnique rdf:resource="https://m82-project.org/dima-bias/ontology#c9ce7d9bb7_vonrestorffeffect_3"/>
  </rdf:Description>
  <rdf:Description rdf:about="https://stratcomcoe.org/influence-mini/ontology#9a2a4d3a26_premise_8">
    <ns1:usesTechnique rdf:resource="https://m82-project.org/dima-bias/ontology#9a2a4d3a26_negativitybias_3"/>
  </rdf:Description>
  <rdf:Description rdf:about="https://stratcomcoe.org/influence-mini/ontology#9a2a4d3a26_argument_2">
    <ns1:usesTechnique rdf:resource="https://m82-project.org/dima-bias/ontology#9a2a4d3a26_vonrestorffeffect_2"/>
    <ns1:usesTechnique rdf:resource="https://m82-project.org/dima-bias/ontology#9a2a4d3a26_hindsightbias_2"/>
  </rdf:Description>
  <rdf:Description rdf:about="https://stratcomcoe.org/influence-mini/ontology#c9ce7d9bb7_premise_0">
    <ns1:usesTechnique rdf:resource="https://m82-project.org/dima-bias/ontology#c9ce7d9bb7_vonrestorffeffect_0"/>
  </rdf:Description>
  <rdf:Description rdf:about="https://stratcomcoe.org/influence-mini/ontology#9a2a4d3a26_development_1">
    <ns1:usesTechnique rdf:resource="https://m82-project.org/dima-bias/ontology#9a2a4d3a26_negativitybias_1"/>
  </rdf:Description>
  <rdf:Description rdf:nodeID="N41749741d84444f2a8f45fafa256c0fc">
    <rdf:type rdf:resource="http://www.w3.org/2002/07/owl#Class"/>
    <owl:intersectionOf rdf:nodeID="N320c12a0b5f04793acfdfb02e53b75c0"/>
  </rdf:Description>
  <rdf:Description rdf:nodeID="Nbc784ea1eddb4b14aac7781fa84aad87">
    <rdf:rest rdf:nodeID="Nd50a1a8a4dbd4010a14d2c09d3d5538d"/>
    <rdf:first rdf:resource="https://stratcomcoe.org/influence-mini/ontology#Argument"/>
  </rdf:Description>
  <rdf:Description rdf:nodeID="N22c16a8180e64cf78cb66d45cbb94d93">
    <rdf:type rdf:resource="http://www.w3.org/2002/07/owl#Class"/>
    <owl:intersectionOf rdf:nodeID="Nbc784ea1eddb4b14aac7781fa84aad87"/>
  </rdf:Description>
  <rdf:Description rdf:about="https://stratcomcoe.org/influence-mini/ontology#c9ce7d9bb7_development_3">
    <ns1:usesTechnique rdf:resource="https://m82-project.org/dima-bias/ontology#c9ce7d9bb7_negativitybias_1"/>
    <ns1:usesTechnique rdf:resource="https://m82-project.org/dima-bias/ontology#c9ce7d9bb7_vonrestorffeffect_1"/>
  </rdf:Description>
  <rdf:Description rdf:about="https://stratcomcoe.org/influence-mini/ontology#c9ce7d9bb7_development_6">
    <ns1:usesTechnique rdf:resource="https://m82-project.org/dima-bias/ontology#c9ce7d9bb7_vonrestorffeffect_4"/>
  </rdf:Description>
  <rdf:Description rdf:about="https://m82-project.org/dima-bias/ontology#9a2a4d3a26_vonrestorffeffect_1">
    <ns1:hasExplanation rdf:datatype="http://www.w3.org/2001/XMLSchema#string">The argument singles out the most recent incident as distinct ('last week's unauthorized...'), making it stand out from the pattern and thus more memorable, exploiting the Von Restorff Effect.</ns1:hasExplanation>
    <rdf:type rdf:resource="http://www.w3.org/2002/07/owl#NamedIndividual"/>
    <rdf:type rdf:resource="https://m82-project.org/dima-bias/ontology#TechniqueUsage"/>
    <ns1:instantiatesTechnique rdf:resource="https://m82-project.org/dima-bias/ontology#VonRestorffEffect"/>
  </rdf:Description>
  <rdf:Description rdf:nodeID="Nac059f911837400bba42ea6c55e0a51d">
    <owl:intersectionOf rdf:nodeID="Nb7abcfaf46464d3e82c7ee49bacb1903"/>
    <rdf:type rdf:resource="http://www.w3.org/2002/07/owl#Class"/>
  </rdf:Description>
  <rdf:Description rdf:about="https://stratcomcoe.org/influence-mini/ontology#c9ce7d9bb7_premise_7">
    <ns1:usesTechnique rdf:resource="https://m82-project.org/dima-bias/ontology#c9ce7d9bb7_negativitybias_4"/>
  </rdf:Description>
  <rdf:Description rdf:nodeID="Nb837f70aaca6452d8df14d0559ef0ec0">
    <rdf:first rdf:nodeID="N6eda40f91b674b0681acd877762669a5"/>
    <rdf:rest rdf:resource="http://www.w3.org/1999/02/22-rdf-syntax-ns#nil"/>
  </rdf:Description>
  <rdf:Description rdf:about="https://stratcomcoe.org/influence-mini/ontology#c9ce7d9bb7_development_7">
    <ns1:usesTechnique rdf:resource="https://m82-project.org/dima-bias/ontology#c9ce7d9bb7_vonrestorffeffect_5"/>
  </rdf:Description>
  <rdf:Description rdf:about="https://stratcomcoe.org/influence-mini/ontology#c9ce7d9bb7_argument_5">
    <ns1:usesTechnique rdf:resource="https://m82-project.org/dima-bias/ontology#c9ce7d9bb7_vonrestorffeffect_5"/>
  </rdf:Description>
  <rdf:Description rdf:about="https://stratcomcoe.org/influence-mini/ontology#9a2a4d3a26_conclusion_0">
    <ns1:usesTechnique rdf:resource="https://m82-project.org/dima-bias/ontology#9a2a4d3a26_vonrestorffeffect_0"/>
  </rdf:Description>
  <rdf:Description rdf:about="https://stratcomcoe.org/influence-mini/ontology#9a2a4d3a26_premise_6">
    <ns1:usesTechnique rdf:resource="https://m82-project.org/dima-bias/ontology#9a2a4d3a26_hindsightbias_2"/>
  </rdf:Description>
</rdf:RDF>
